<?xml version="1.0" encoding="UTF-8" ?>

<!-- Copyright 2018 Joel Feldman, Andrew Rechnitzer and Elyse Yeager -->
<!-- This work is licensed under the Creative Commons Attribution-NonCommercial-ShareAlike 4.0 International License-->
<!-- https://creativecommons.org/licenses/by-nc-sa/4.0 -->

<exercises>
<exercisegroup>
<introduction><conceptual/></introduction>

<exercise>
<statement><p>
Let <m>0 \lt \theta \lt \frac{\pi}{2}</m>, and <m>a,b \gt 0</m>. Denote by <m>S</m> the part of
the surface <m>z=y\,\tan\theta</m> with <m>0\le x\le a</m>, <m>0\le y\le b</m>.
<ol marker="a">
<li>
Find the surface area of <m>S</m> without using any calculus.
</li>
<li>
Find the surface area of <m>S</m> by using Theorem <xref ref="thm_surface_area"/>.
</li>
</ol>
</p>

</statement>

<hint><p>
<m>S</m> is a very simple geometric object.
</p></hint>

<answer><p>
<m>ab\sqrt{1+\tan^2\theta}=ab\sec\theta</m>
</p></answer>

<solution><p>
(a) <m>S</m> is the part of the plane <m>z=y\,\tan\theta</m> that lies above the
rectangle in the <m>xy</m>-plane with vertices <m>(0,0)</m>, <m>(a,0)</m>, <m>(0,b)</m>, <m>(a,b)</m>.
So <m>S</m> is the rectangle with vertices <m>(0,0,0)</m>,
<m>(a,0,0)</m>, <m>(0,b,b\tan\theta)</m>, <m>(a,b,b\tan\theta)</m>. So it has side lengths
<md>
<mrow>
|\llt a,0,0\rgt -\llt 0,0,0\rgt| &amp;=a
</mrow><mrow>
|\llt 0,b,b\tan\theta\rgt -\llt 0,0,0\rgt| &amp;=  \sqrt{b^2+b^2\tan^2\theta}
</mrow>
</md>
and hence area <m>ab\sqrt{1+\tan^2\theta}=ab\sec\theta</m>.
</p>

<p>(b) <m>S</m> is the part of the surface <m>z=f(x,y)</m> with <m>f(x,y) = y\,\tan\theta</m>
and with <m>(x,y)</m> running over
<me>
\cD =\Set{(x,y)}{0\le x\le a,\ 0\le y\le b}
</me>
Hence by Theorem <xref ref="thm_surface_area"/>
<md>
<mrow>
\text{Area}(S)&amp;=\dblInt_\cD \sqrt{1+f_x(x,y)^2+f_y(x,y)^2}\ \dee{x}\,\dee{y}
</mrow><mrow>
&amp;=\int_0^a\dee{x}\int_0^b\dee{y}\ \sqrt{1+0^2+\tan^2\theta}
</mrow><mrow>
&amp;=ab\sqrt{1+\tan^2\theta}=ab\sec\theta
</mrow>
</md>
</p>

</solution>
</exercise>

<exercise>
<statement><p>
Let <m>c  \gt  0</m>. Denote by <m>S</m> the part of
the surface <m>ax+by+cz=d</m> with <m>(x,y)</m> running over the region <m>D</m> in the <m>xy</m>-plane.
Find the surface area of <m>S</m>, in terms of <m>a</m>, <m>b</m>, <m>c</m>, <m>d</m> and <m>A(D)</m>,
the area of the region <m>D</m>.
</p></statement>

<answer><p>
<m>\frac{\sqrt{a^2+b^2+c^2}}{c} A(D)</m>
</p></answer>

<solution><p>
 <m>S</m> is the part of the surface <m>z=f(x,y)</m> with <m>f(x,y) = \frac{d-ax-by}{c}</m>
and with <m>(x,y)</m> running over <m>D</m>.
Hence by Theorem <xref ref="thm_surface_area"/>
<md>
<mrow>
\text{Area}(S)&amp;=\dblInt_D \sqrt{1+f_x(x,y)^2+f_y(x,y)^2}\ \dee{x}\,\dee{y}
</mrow><mrow>
&amp;=\dblInt_D\ \sqrt{1+\frac{a^2}{c^2}+\frac{b^2}{c^2}}
</mrow><mrow>
&amp;=\frac{\sqrt{a^2+b^2+c^2}}{c} A(D)
</mrow>
</md>
</p>

</solution>
</exercise>

<exercise>
<statement><p>
Let <m>a,b,c  \gt  0</m>. Denote by <m>S</m> the triangle with vertices <m>(a,0,0)</m>,
<m>(0,b,0)</m> and <m>(0,0,c)</m>.
<ol marker="a">
<li>
Find the surface area of <m>S</m> in three different ways, each using
Theorem <xref ref="thm_surface_area"/>.
</li>
<li>
Denote by <m>T_{xy}</m> the projection of <m>S</m> onto the <m>xy</m>-plane. (It is the
triangle with vertices <m>(0,0,0)</m> <m>(a,0,0)</m> and <m>(0,b,0)</m>.) Similarly use
<m>T_{xz}</m> to denote the projection of <m>S</m> onto the <m>xz</m>-plane and
<m>T_{yz}</m> to denote the projection of <m>S</m> onto the <m>yz</m>-plane. Show that
<me>
\text{Area}(S) =\sqrt{\text{Area}(T_{xy})^2
                     +\text{Area}(T_{xz})^2
                     +\text{Area}(T_{yz})^2
                     }
</me>
</li>
</ol>
</p></statement>

<hint><p>
The triangle is part of the plane <m>\frac{x}{a}+\frac{y}{b} +\frac{z}{c}=1</m>.
</p></hint>

<answer><p>
(a) <m>\frac{1}{2}\sqrt{a^2b^2+a^2c^2+b^2c^2}</m>
</p>

<p>(b) See the solution.
</p></answer>

<solution><p>
Note that all three vertices <m>(a,0,0)</m>, <m>(0,b,0)</m> and <m>(0,0,c)</m> lie on
the plane <m>\frac{x}{a}+\frac{y}{b} +\frac{z}{c}=1</m>. So the triangle is
part of that plane.
</p>

<p><em>Method 1.</em>
 <m>S</m> is the part of the surface <m>z=f(x,y)</m> with
<m>f(x,y) = c\left(1-\frac{x}{a}-\frac{y}{b}\right)</m>
and with <m>(x,y)</m> running over the triangle <m>T_{xy}</m> in the <m>xy</m>-plane
with vertices <m>(0,0,0)</m> <m>(a,0,0)</m> and <m>(0,b,0)</m>.
Hence by part a of Theorem <xref ref="thm_surface_area"/>
<md>
<mrow>
\text{Area}(S)&amp;=\dblInt_{T_{xy}} \sqrt{1+f_x(x,y)^2+f_y(x,y)^2}\ \dee{x}\,\dee{y}
</mrow><mrow>
&amp;=\dblInt_{T_{xy}}\ \sqrt{1+\frac{c^2}{a^2}+\frac{c^2}{b^2}}\
\dee{x}\,\dee{y}
</mrow><mrow>
&amp;=\sqrt{1+\frac{c^2}{a^2}+\frac{c^2}{b^2}}\ A(T_{xy})
</mrow>
</md>
where <m>A(T_{xy})</m> is the area of <m>T_{xy}</m>. Since the triangle <m>T_{xy}</m>
has base <m>a</m> and height <m>b</m> (see the figure below), it has
area <m>\frac{1}{2}ab</m>. So
<me>
\text{Area}(S)=\frac{1}{2}\sqrt{1+\frac{c^2}{a^2}+\frac{c^2}{b^2}}\ ab
 =\frac{1}{2}\sqrt{a^2b^2+a^2c^2+b^2c^2}
</me>
</p>

<sidebyside width="45%">
  <image source="pfigs/triangleProjection"/>
</sidebyside>

<p>
<em>Method 2.</em>
 <m>S</m> is the part of the surface <m>x=g(y,z)</m> with
<m>g(y,z) = a\left(1-\frac{y}{b}-\frac{z}{c}\right)</m>
and with <m>(y,z)</m> running over the triangle <m>T_{yz}</m> in the <m>yz</m>-plane
with vertices <m>(0,0,0)</m> <m>(0,b,0)</m> and <m>(0,0,c)</m>.
Hence by part b of Theorem <xref ref="thm_surface_area"/>
<md>
<mrow>
\text{Area}(S)&amp;=\dblInt_{T_{yz}} \sqrt{1+g_y(y,z)^2+g_z(y,z)^2}\ \dee{y}\,\dee{z}
</mrow><mrow>
&amp;=\dblInt_{T_{yz}}\ \sqrt{1+\frac{a^2}{b^2}+\frac{a^2}{c^2}}\
\dee{y}\,\dee{z}
</mrow><mrow>
&amp;=\sqrt{1+\frac{a^2}{b^2}+\frac{a^2}{c^2}}\ A(T_{yz})
</mrow>
</md>
where <m>A(T_{yz})</m> is the area of <m>T_{yz}</m>. Since <m>T_{yz}</m> has base <m>b</m> and
height <m>c</m>, it has area <m>\frac{1}{2}bc</m>. So
<me>
\text{Area}(S)=\frac{1}{2}\sqrt{1+\frac{a^2}{b^2}+\frac{a^2}{c^2}}\ bc
 =\frac{1}{2}\sqrt{a^2b^2+a^2c^2+b^2c^2}
</me>
</p>

<p><em>Method 3.</em>
 <m>S</m> is the part of the surface <m>y=h(x,z)</m> with
<m>h(x,z) = b\left(1-\frac{x}{a}-\frac{z}{c}\right)</m>
and with <m>(x,z)</m> running over the triangle <m>T_{xz}</m> in the <m>xz</m>-plane
with vertices <m>(0,0,0)</m> <m>(a,0,0)</m> and <m>(0,0,c)</m>.
Hence by part c of Theorem <xref ref="thm_surface_area"/>
<md>
<mrow>
\text{Area}(S)&amp;=\dblInt_{T_{xz}} \sqrt{1+h_x(x,z)^2+h_z(x,z)^2}\ \dee{x}\,\dee{z}
</mrow><mrow>
&amp;=\dblInt_{T_{xz}}\ \sqrt{1+\frac{b^2}{a^2}+\frac{b^2}{c^2}}\
\dee{x}\,\dee{z}
</mrow><mrow>
&amp;=\sqrt{1+\frac{b^2}{a^2}+\frac{b^2}{c^2}}\ A(T_{xz})
</mrow>
</md>
where <m>A(T_{xz})</m> is the area of <m>T_{xz}</m>. Since <m>T_{xz}</m> has base <m>a</m> and
height <m>c</m>, it has area <m>\frac{1}{2}ac</m>. So
<me>
\text{Area}(S)=\frac{1}{2}\sqrt{1+\frac{b^2}{a^2}+\frac{b^2}{c^2}}\ bc
 =\frac{1}{2}\sqrt{a^2b^2+a^2c^2+b^2c^2}
</me>
</p>

<p>(b) We have already seen in the solution to part (a) that
<me>
\text{Area}(T_{xy})=\frac{ab}{2}\qquad
\text{Area}(T_{xz})=\frac{ac}{2}\qquad
\text{Area}(T_{yz})=\frac{bc}{2}\qquad
</me>
Hence
<md>
<mrow>
\text{Area}(S)
&amp;=\sqrt{\frac{a^2b^2}{4}+\frac{a^2c^2}{4}+\frac{b^2c^2}{4}}
</mrow><mrow>
&amp;=\sqrt{\text{Area}(T_{xy})^2
                     +\text{Area}(T_{xz})^2
                     +\text{Area}(T_{yz})^2
                     }
</mrow>
</md>
</p>

</solution>
</exercise>
</exercisegroup>

<exercisegroup><introduction><procedural/></introduction>

<exercise><title><fromexam>M317 2002A</fromexam></title>
<statement><p>
 Find the area of the part of the surface <m>z=y^{3/2}</m> that
lies above <m>0\le x,y\le 1</m>.
</p></statement>

<answer><p>
<m>\frac{8}{27}\left[\left(\frac{13}{4}\right)^{3/2}-1\right]</m>
</p></answer>

<solution><p>
For the surface <m>z=f(x,y)=y^{3/2}</m>,
<me>
\dee{S}=\sqrt{1+f_x^2+f_y^2}\ \dee{x}\dee{y}
=\sqrt{1+\Big(\frac{3}{2}\sqrt{y}\Big)^2}\ \dee{x}\dee{y}
=\sqrt{1+\frac{9}{4}y}\ \dee{x}\dee{y}
</me>
by Theorem <xref ref="thm_surface_area"/>.a,
So the area is
<md>
<mrow>
\int_0^1\dee{x}\int_0^1\dee{y}\ \sqrt{1+\frac{9}{4}y}
&amp;=\int_0^1\dee{x}\ \frac{8}{27}\Big[\Big(1+\frac{9}{4}y\Big)^{3/2}\Big]_0^1
</mrow><mrow>
&amp;=\int_0^1\dee{x}\ \frac{8}{27}\Big[\Big(\frac{13}{4}\Big)^{3/2}-1\Big]
</mrow><mrow>
&amp;=\frac{8}{27}\left[\left(\frac{13}{4}\right)^{3/2}-1\right]
</mrow>
</md>
</p></solution>
</exercise>

<exercise><title><fromexam>M253 2013D</fromexam></title>
<statement><p>
Find the surface area of the part of the paraboloid
<m>z = a^2 - x^2 - y^2</m> which lies above the <m>xy</m>--plane.
</p></statement>

<answer><p>
<m>\frac{\pi}{6}\big[{(1+4a^2)}^{3/2}-1\big]</m>
</p></answer>

<solution><p>
First observe that any point <m>(x,y,z)</m> on the paraboliod lies above the <m>xy</m>-plane if and only if
<me>
0\le z = a^2-x^2-y^2
\iff x^2+y^2\le a^2
</me>
That is, if and only if <m>(x,y)</m> lies in the circular disk of radius <m>a</m>
centred on the origin. The equation of the paraboloid is of the form
<m>z=f(x,y)</m> with <m>f(x,y)=a^2-x^2-y^2</m>. So, by
Theorem <xref ref="thm_surface_area"/>.a,
<md>
<mrow>
\text{Surface area}
&amp;= \dblInt_{x^2+y^2\le a^2}\sqrt{1+f_x(x,y)^2+f_y(x,y)^2}\ \dee{x}\,\dee{y}
</mrow><mrow>
&amp;= \dblInt_{x^2+y^2\le a^2}\sqrt{1+4x^2+4y^2}\ \dee{x}\,\dee{y}
</mrow>
</md>
Switching to polar coordinates,
<md>
<mrow>
\text{Surface area}
&amp;= \int_0^a\dee{r}\int_0^{2\pi}\dee{\theta}\ r\sqrt{1+4r^2}
</mrow><mrow>
&amp;= 2\pi \int_0^a\dee{r}\ r\sqrt{1+4r^2}
</mrow><mrow>
&amp;= 2\pi \int_1^{1+4a^2}\frac{\dee{s}}{8}\ \sqrt{s}\qquad
\text{with } s=1+4r^2, \dee{s}=8r\,\dee{r}
</mrow><mrow>
&amp;=\frac{\pi}{4}\ \frac{2}{3}s^{3/2}\bigg|_{s=1}^{s=1+4a^2}
</mrow><mrow>
&amp;=\frac{\pi}{6}\big[{(1+4a^2)}^{3/2}-1\big]
</mrow>
</md>
</p>

</solution>
</exercise>

<exercise><title><fromexam>M253 2014D</fromexam></title>
<statement><p>
Find the area of the portion of the cone <m>z^2 = x^2 + y^2</m>
lying between the planes <m>z = 2</m> and <m>z = 3</m>.
</p></statement>

<answer><p>
<m>5\sqrt{2}\pi</m>
</p></answer>

<solution><p>
First observe that any point <m>(x,y,z)</m> on the cone lies between the
planes <m>z=2</m> and <m>z=3</m> if and only if <m>4\le x^2+y^2\le 9</m>.
</p>

<p>The equation of the cone can be rewritten in the form
<m>z=f(x,y)</m> with <m>f(x,y)=\sqrt{x^2+y^2}</m>. Note that
<md>
<mrow>
f_x(x,y)=\frac{x}{\sqrt{x^2+y^2}}\qquad
f_y(x,y)=\frac{y}{\sqrt{x^2+y^2}}
</mrow>
</md>
So, by
Theorem <xref ref="thm_surface_area"/>.a,
<md>
<mrow>
\text{Surface area}
&amp;= \dblInt_{4\le x^2+y^2\le 9}\sqrt{1+f_x(x,y)^2+f_y(x,y)^2}\ \dee{x}\,\dee{y}
</mrow><mrow>
&amp;= \dblInt_{4\le x^2+y^2\le 9}
    \sqrt{1+\frac{x^2}{x^2+y^2}+\frac{y^2}{x^2+y^2}}\ \dee{x}\,\dee{y}
</mrow><mrow>
&amp;=\sqrt{2} \dblInt_{4\le x^2+y^2\le 9} \dee{x}\,\dee{y}
</mrow>
</md>
Now the domain of integration is a circular washer with outside radius <m>3</m>
and inside radius <m>2</m> and hence of area <m>\pi(3^2-2^2)=5\pi</m>. So the surface area is <m>5\sqrt{2}\pi</m>.
</p>

</solution>
</exercise>

<exercise><title><fromexam>M253 2015D</fromexam></title>
<statement><p>
Determine the surface area of the surface given by
<m>z = \frac{2}{3}\big(x^{3/2} + y^{3/2}\big)</m>, over the square
<m>0 \le  x \le  1</m>, <m>0 \le  y \le  1</m>.
</p></statement>

<answer><p>
<m>\frac{4}{15}\big[9\sqrt{3}-8\sqrt{2}+1\big]</m>
</p></answer>

<solution><p>
The equation of the surface is of the form
<m>z=f(x,y)</m> with <m>f(x,y)=\frac{2}{3}\big(x^{3/2} + y^{3/2}\big)</m>. Note that
<md>
<mrow>
f_x(x,y)=\sqrt{x}\qquad
f_y(x,y)=\sqrt{y}
</mrow>
</md>
So, by Theorem <xref ref="thm_surface_area"/>.a,
<md>
<mrow>
\text{Surface area}
&amp;= \int_0^1\dee{x}\int_0^1\dee{y}\ \sqrt{1+f_x(x,y)^2+f_y(x,y)^2}
</mrow><mrow>
&amp;= \int_0^1\dee{x}\int_0^1\dee{y}\ \sqrt{1+x+y}
</mrow><mrow>
&amp;= \int_0^1\dee{x}\ \Big[\frac{2}{3}(1+x+y)^{3/2}\Big]_{y=0}^{y=1}
</mrow><mrow>
&amp;= \frac{2}{3}\int_0^1\dee{x}\ \big[(2+x)^{3/2}-(1+x)^{3/2}\big]
</mrow><mrow>
&amp;= \frac{2}{3}\ \frac{2}{5}\Big[(2+x)^{5/2}-(1+x)^{5/2}\Big]_{x=0}^{x=1}
</mrow><mrow>
&amp;= \frac{4}{15} \big[3^{5/2}-2^{5/2}-2^{5/2}+1^{5/2}\big]
</mrow><mrow>
&amp;= \frac{4}{15}\big[9\sqrt{3}-8\sqrt{2}+1\big]
</mrow>
</md>
</p></solution>
</exercise>

<exercise><title><fromexam>M253 2016D</fromexam></title>
<statement><p>
<ol marker="a">
<li>
To find the surface area of the surface <m>z = f (x,y)</m> above the region <m>D</m>,
we integrate <m>\dblInt_D F(x,y)\ \dee{A}</m>. What is <m>F(x,y)</m>?
</li>
<li>
<p>
Consider a <q>Death Star</q>,  a ball of radius <m>2</m> centred at the origin
with another ball of radius <m>2</m> centred at <m>(0, 0, 2\sqrt{3})</m> cut out of it.
The diagram below shows the slice where <m>y = 0</m>.
</p>

<sidebyside width="50%">
  <image source="pfigs/OE253_16D_2"/>
</sidebyside>
<p>
<ol marker="(i)">
<li>
The Rebels want to paint part of the surface of Death Star hot pink; specifically, the concave part (indicated with a thick line in the diagram).
To help them determine how much paint is needed, carefully fill in the
missing parts of this integral:
<me>
\text{surface area} =
\int_{\underline{\ \ \ \ }}^{\underline{\ \ \ \ }}
                 \int_{\underline{\ \ \ \ }}^{\underline{\ \ \ \ }}
                        \underline{\ \ \ \ \ \ \ \ \ \ }\ \dee{r}\,\dee{\theta}
</me>
</li>
<li>
What is the total surface area of the Death Star?
</li>
</ol></p>
</li>
</ol>
</p></statement>

<hint><p>
The total surface area of (b) (ii) can be determined without evaluating
any integrals.
</p></hint>

<answer><p>
(a)  <m>F(x,y) = \sqrt{1+f_x(x,y)^2+f_y(x,y)^2}</m>
</p><p>
(b)-(i) <m>\int_0^{2\pi}\dee{\theta}\int_0^1\dee{r}\ \frac{2r}{\sqrt{4-r^2}}</m>
</p><p>
(b)-(ii) <m>16\pi</m>
</p></answer>

<solution><p>
(a)
By Theorem <xref ref="thm_surface_area"/>.a,
<m>F(x,y) = \sqrt{1+f_x(x,y)^2+f_y(x,y)^2}</m>.
</p>

<p>(b)  (i) The <q>dimple</q> to be painted is part of the upper sphere
<m>x^2+y^2+\big(z-2\sqrt{3}\big)^2=4</m>. It is on the bottom half of the sphere
and so has equation <m>z=f(x,y)=2\sqrt{3}-\sqrt{4-x^2-y^2}</m>. Note that
<md>
<mrow>
f_x(x,y) = \frac{x}{\sqrt{4-x^2-y^2}}\qquad
f_y(x,y) = \frac{y}{\sqrt{4-x^2-y^2}}
</mrow>
</md>
The point on the dimple with the largest value of <m>x</m> is
<m>(1,0,\sqrt{3})</m>. (It is marked by a dot in the figure above.) The dimple
is invariant under rotations around the <m>z</m>--axis and so has <m>(x,y)</m>
running over <m>x^2+y^2\le 1</m>. So, by
Theorem <xref ref="thm_surface_area"/>.a,
<md>
<mrow>
\text{Surface area}
&amp;= \dblInt_{x^2+y^2\le 1}\sqrt{1+f_x(x,y)^2+f_y(x,y)^2}\ \dee{x}\,\dee{y}
</mrow><mrow>
&amp;= \dblInt_{x^2+y^2\le 1}\sqrt{1+\frac{x^2}{4-x^2-y^2}
                                +\frac{y^2}{4-x^2-y^2}}\ \dee{x}\,\dee{y}
</mrow><mrow>
&amp;= \dblInt_{x^2+y^2\le 1}\frac{2}{\sqrt{4-x^2-y^2}}\ \dee{x}\,\dee{y}
</mrow>
</md>
Switching to polar coordinates,
<md>
<mrow>
\text{Surface area}
&amp;= \int_0^{2\pi}\dee{\theta}\int_0^1\dee{r}\ \frac{2r}{\sqrt{4-r^2}}
</mrow>
</md>
</p>

<p>(b) (ii) Observe that if we flip the dimple up by reflecting it
in the plane <m>z=\sqrt{3}</m>, as in the figure below, the <q>Death Star</q>
becomes a perfect ball of radius <m>2</m>.
</p>
<sidebyside width="50%">
  <image source="pfigs/OE253_16D_2a"/>
</sidebyside>
<p>
The area of the pink dimple in the figure above is identical to the area
of the blue cap in that figure. So the total surface area of the
Death Star is exactly the surface area of a sphere of radius <m>a=2</m> and so
(see Example <xref ref="eg_area_hemisphere"/>)
is <m>4\pi a^2 = 4 \pi 2^2=16\pi</m>.
</p>

</solution>
</exercise>

<exercise>
<statement><p> 
Find the area of the part of the cone <m>x^2=3y^2+3z^2</m> between <m>x=\sqrt{3}</m> and <m>x=2\sqrt{3}</m>.
</p></statement>

<hint><p>
Rewrite the equation of the cone in the form <m>x=g(y,z)</m>.
</p></hint>

<answer><p>
<m>6\pi\approx 18.85</m>
</p></answer>

<solution><p>
The equation of the half of the cone with <m>x\ge 0</m> can be rewritten in the form 
<m>x=g(y,z)</m> with <m>g(y,z)=\sqrt{3}\sqrt{y^2+z^2}</m>. Note that
<me>
g_y(y,z)=\frac{\sqrt{3}y}{\sqrt{y^2+z^2}}\quad
g_z(y,z)=\frac{\sqrt{3}z}{\sqrt{y^2+z^2}}
</me>
so that, by Theorem <xref ref="thm_surface_area"/>,
<md>
<mrow>
\dee{S}&amp;=\sqrt{1+g_y(y,z)^2+g_z(y,z)^2}\,\dee{y}\,\dee{z}
</mrow><mrow>
&amp;=\sqrt{1+\frac{3y^2}{y^2+z^2}+\frac{3z^2}{y^2+z^2}}\,\dee{y}\,\dee{z}
</mrow><mrow>
&amp;=2\,\dee{y}\,\dee{z}
</mrow>
</md>
A point <m>(x,y,z)</m> on <m>x=\sqrt{3}\sqrt{y^2+z^2}</m> has <m>\sqrt{3}\le x\le 2\sqrt{3}</m> if and only if
<m>1\le\sqrt{y^2+z^2}\le 2</m>. So
<md>
<mrow>
&amp;\text{Area}= \dblInt_{1\le \sqrt{y^2+z^2}\le 2}2\,\dee{y}\,\dee{z} 
</mrow><mrow>
&amp;\hskip0.25in=2\,\Big[\text{area of }\Set{(y,z)}{\sqrt{y^2+z^2}\le 2}-
           \text{area of }\Set{(y,z)}{\sqrt{y^2+z^2}\le 1}\Big]
</mrow><mrow>
&amp;\hskip0.25in=2\,\big[\pi 2^2-\pi 1^2\big]
=6\pi\approx 18.85
</mrow>
</md>
</p></solution>
</exercise>

<exercise><title><fromexam>M200 2001D</fromexam></title>
<statement><p> 
Find the surface area of that part of the hemisphere
<m>z=\sqrt{a^2-x^2-y^2}</m> which lies within the cylinder <m>\big(x-\frac{a}{2}\big)^2+y^2=\big(\frac{a}{2}\big)^2</m>.
</p></statement>

<answer><p>
<m>a^2[\pi-2]</m>
</p></answer>

<solution><p>
We are to find the surface area of part of a hemisphere. On the hemisphere
<md>
<mrow>
z=f(x,y)&amp;=\sqrt{a^2-x^2-y^2}
</mrow><mrow>
f_x(x,y)&amp;=-\frac{x}{\sqrt{a^2-x^2-y^2}}\qquad
f_y(x,y)=-\frac{y}{\sqrt{a^2-x^2-y^2}}
</mrow>
</md>
so that
<md>
<mrow>
\dee{S}&amp;=\sqrt{1+f_x(x,y)^2+f_y(x,y)^2}\,\dee{x}\,\dee{y}
</mrow><mrow>
&amp;=\sqrt{1+\frac{x^2}{a^2-x^2-y^2}+\frac{y^2}{a^2-x^2-y^2}}\,\dee{x}\,\dee{y}
</mrow><mrow>
&amp;=\sqrt{\frac{a^2}{a^2-x^2-y^2}}\,\dee{x}\,\dee{y}
</mrow>
</md>
In polar coordinates, this is <m>\dee{S}=\frac{a}{\sqrt{a^2-r^2}}\,r\,\dee{r}\,\dee{\theta}</m>.
We are to find the surface area of the part of the hemisphere that is
inside the cylinder, <m>x^2-ax+y^2=0</m>, which is polar coordinates is
becomes <m>r^2-ar\cos\theta=0</m> or <m>r=a\cos\theta</m>. The top half of the domain of
integration is sketched below.
</p>
<sidebyside width="50%">
  <image source="pfigs/OE01DQ7"/>
</sidebyside>
<p>
So the
<md>
<mrow>
{\rm Surface\ Area}
&amp;= 2\int_0^{\pi/2}\dee{\theta}\int_0^{a\cos\theta}\dee{r}\ r
                                      \frac{a}{\sqrt{a^2-r^2}}
</mrow><mrow>
&amp;= 2a\int_0^{\pi/2}\dee{\theta}\ \Big[-\sqrt{a^2-r^2}\,\Big]_0^{a\cos\theta}
</mrow><mrow>
&amp;= 2a\int_0^{\pi/2}\dee{\theta}\ \big[a-a\sin\theta\big]
</mrow><mrow>
&amp;= 2a^2\Big[\theta+\cos\theta\Big]_0^{\pi/2}
=a^2[\pi-2]
</mrow>
</md>
</p></solution>
</exercise></exercisegroup>

</exercises>
