<?xml version="1.0" encoding="UTF-8" ?>
<!-- Copyright 2018-2020 Joel Feldman, Andrew Rechnitzer and Elyse Yeager -->
<!-- This work is licensed under the Creative Commons Attribution-NonCommercial-ShareAlike 4.0 International License-->
<!-- https://creativecommons.org/licenses/by-nc-sa/4.0 -->

<section xmlns:xi="http://www.w3.org/2001/XInclude" xml:id="sec_lines_3d">
  <title>Equations of Lines in 3d</title>

  <p>Just as in two dimensions, a line in three dimensions can be specified  by
  giving one point <m>(x_0,y_0,z_0)</m> on the line and one vector
  <m>\vd=\llt d_x,d_y,d_z\rgt </m> whose direction is parallel to that of the line.
  If <m>(x,y,z)</m> is any point on the line then the vector <m>\llt x-x_0,y-y_0,z-z_0\rgt </m>,
  whose tail is at <m>(x_0,y_0,z_0)</m> and whose arrow is at <m>(x,y,z)</m>,  must be
  parallel to <m>\vd</m> and hence a scalar multiple of <m>\vd</m>. By translating
  this statement into a vector equation we get
</p>

<fact xml:id="par_eqn_of_line"><title>Parametric Equations of a Line</title>
<p>
  <md>
  <mrow>
  \llt x-x_0,y-y_0,z-z_0\rgt =t \vd
  </mrow>
  </md>
  or the three corresponding scalar equations
  <md>
  <mrow>
  x-x_0 = t d_x\qquad
  y-y_0 = t d_y\qquad
  z-z_0 = t d_z
  </mrow>
  </md>
</p>
</fact>

<p>
  again gives the parametric equations of the plane.
  Solving all three equations for the parameter <m>t</m>
  <md>
  <mrow>
  t=\frac{x-x_0}{d_x}=\frac{y-y_0}{d_y}=\frac{z-z_0}{d_z}
  </mrow>
  </md>
  and erasing the <q><m>t=</m></q> again gives the (so called) symmetric
  equations for the line.
  </p>

<example xml:id="eg_line_equations">
  <p>
  The set of points <m>(x,y,z)</m> that obey <m>x+y+z=2</m> form a
  plane. The set of points <m>(x,y,z)</m> that obey <m>x-y=0</m> form a second plane.
   The set of points <m>(x,y,z)</m> that obey both <m>x+y+z=2</m> and <m>x-y=0</m>  lie
  on the intersection of these two planes and hence form a line. We shall
  find the parametric equations for that line.
  </p>

  <p>To sketch <m>x+y+z=2</m> we observe
  that if any two of <m>x,y,z</m> are zero, then the third is <m>2</m>. So all of <m>(0,0,2)</m>,
  <m>(0,2,0)</m> and <m>(2,0,0)</m> are on <m>x+y+z=2</m>. The plane <m>x-y=0</m> contains all
  of the <m>z</m>-axis, since <m>(0,0,z)</m> obeys <m>x-y=0</m> for all <m>z</m>.
  Here are separate sketches of (parts of) the two planes.
</p>

<sidebyside widths="50% 40%" valign="middle">
<image source="figs/planeIntA"/>
<image source="figs/planeIntB"/>
</sidebyside>

<p>
  And here is a sketch of their intersection
</p>

<sidebyside width="50%">
<image source="figs/planeInt"/>
</sidebyside>

<p>
  <em>Method 1.</em> Each point on the line has a different value of
  <m>z</m>. We'll use <m>z</m> as the parameter. (We could just as well use <m>x</m> or
  <m>y</m>.) There is no law that requires us to use the parameter name <m>t</m>,
  but that's what we have done so far, so set <m>t=z</m>. If <m>(x,y,z)</m> is on
  the line then <m>z=t</m> and
  <md>
  <mrow>
  x+y+t&amp;=2
  </mrow><mrow>
  x-y\phantom{\ \,+t}&amp;=0
  </mrow><mrow>
  </mrow>
  </md>
  The second equation forces <m>y=x</m>. Substituting this into the first equation
  gives
  <md>
  <mrow>
  2x+t=2 \implies x=y=1-\tfrac{t}{2}
  </mrow>
  </md>
  So the parametric equations are
  <md>
  <mrow>
  x=1-\frac{t}{2},\
  y=1-\frac{t}{2},\
  z=t\qquad\text{or}\qquad
  \llt x-1,y-1,z\rgt  = t\llt -\frac{1}{2}, -\frac{1}{2}, 1\rgt
  </mrow>
  </md>
  </p>

  <p>
    <em>Method 2.</em> We first find one point on the line. There
  are lots of them. We'll find the point with <m>z=0</m>. (We could just as well
  use z=123.4, but arguably <m>z=0</m> is a little easier.) If  <m>(x,y,z)</m> is
  on the line and <m>z=0</m>, then
  <md>
  <mrow>
  x+y&amp;=2
  </mrow><mrow>
  x-y&amp;=0
  </mrow>
  </md>
  The second equation forces again <m>y=x</m>. Substituting this into the first
  equation gives
  <md>
  <mrow>
  2x=2 \implies x=y=1
  </mrow>
  </md>
  So <m>(1,1,0)</m> is on the line. Now we'll find a direction vector, <m>\vd</m>,
  for the line. Since the line is contained in the plane <m>x+y+z=2</m>,
  any vector lying on the line, like <m>\vd</m>, is also completely contained
  in that plane. So <m>\vd</m> must be perpendicular to the normal vector of
  <m>x+y+z=2</m>, which is <m>\llt 1,1,1\rgt </m>. Similarly, since the line is
  contained in the plane <m>x-y=0</m>, any vector lying on the line, like <m>\vd</m>, is also completely contained in that plane.  So <m>\vd</m> must be perpendicular to
  the normal vector of <m>x-y=0</m>, which is <m>\llt 1,-1,0\rgt </m>. So we may choose for
  <m>\vd</m> any vector which is perpendicular to both <m>\llt 1,1,1\rgt </m> and
  <m>\llt 1,-1,0\rgt</m>, like, for example,
  <md>
  <mrow>
  \vd&amp;=\llt 1,-1,0\rgt \times\llt 1,1,1\rgt
  </mrow>
  <mrow>
  &amp; =\det\left[ \begin{matrix}\hi &amp;\hj&amp;\hk
  </mrow><mrow> 1&amp;-1&amp;0\\ 1&amp;1&amp;1\end{matrix}\right]
  =\hi\det\left[\begin{matrix}-1&amp;0
  </mrow><mrow>1&amp;1\end{matrix}\right]
  -\hj\det\left[\begin{matrix}1&amp;0
  </mrow><mrow> 1&amp;1\end{matrix}\right]
  +\hk\det\left[\begin{matrix}1&amp;-1
  </mrow><mrow> 1&amp;1\end{matrix}\right]\\
  &amp;=-\hi-\hj+2\hk
  </mrow>
  </md>
  We now have both a point on the line and a direction vector for the line,
  so, as usual, the parametric equations for the line are
  <md>
  <mrow>
  \llt x-1,y-1,z\rgt =t\llt -1,-1,2\rgt \qquad\text{or}\qquad
  x=1-t,\ y=1-t,\ z=2t
  </mrow>
  </md>
  This looks a little different than the solution from method 1, but we'll see in a moment that they are really the same. Before that, let's do one more method.
  </p>

  <p>
    <em>Method 3.</em> We'll find two points on the line. We
  have already found that <m>(1,1,0)</m> is on the line. From the picture above,
  it looks like <m>(0,0,2)</m> is also on the line. This is indeed the case
  since <m>(0,0,2)</m> obeys both <m>x+y+z=2</m> and <m>x-y=0</m>. Notice that we could also have
  guessed <m>(0,0,2)</m> by setting <m>x=0</m>  and then solving <m>y+z=x+y+z=2</m>, <m>-y=x-y=0</m>
  for <m>x</m> and <m>y</m>. As both <m>(1,1,0)</m>
  and <m>(0,0,2)</m> are on the line, the vector with head at <m>(1,1,0)</m> and tail
  at <m>(0,0,2)</m>, which is <m>\llt 1-0,1-0,0-2\rgt =\llt 1,1,-2\rgt </m>, is a direction vector for the
  line. As <m>(0,0,2)</m> is a point on the line and <m>\llt 1,1,-2\rgt </m> is a direction
  vector for the line, the parametric equations for the line are
  <md>
  <mrow>
  \llt x-0,y-0,z-2\rgt =t\llt 1,1,-2\rgt \qquad\text{or}\qquad
  x=t,\ y=t,\ z=2-2t
  </mrow>
  </md>
  This also looks similar, but not quite identical, to our previous answers.
  Time for a comparison.
  </p>

  <p>
    <em>Comparing the answers.</em>
  The parametric equations given by the three methods are different. That's
  just because we have really used different parameters in the three methods,
  even though we have called the parameter <m>t</m> in each case.
  To clarify the relation
  between the three answers, rename the parameter of method 1 to <m>t_1</m>,
  the parameter of method 2 to <m>t_2</m> and the parameter of method 3 to <m>t_3</m>.
  The parametric equations then become
  <md alignment="alignat">
  <mrow>
  &amp;\text{Method 1:}\qquad &amp;
     x&amp;=1-\frac{t_1}{2}\qquad &amp;
     y&amp;=1-\frac{t_1}{2}\qquad &amp;
     z&amp;=t_1
  </mrow><mrow>
  &amp;\text{Method 2:}\qquad &amp;
     x&amp;=1-t_2\qquad &amp;
     y&amp;=1-t_2\qquad &amp;
     z&amp;=2t_2
  </mrow><mrow>
  &amp;\text{Method 3:}\qquad &amp;
     x&amp;=t_3\qquad &amp;
     y&amp;=t_3\qquad &amp;
     z&amp;=2-2t_3
  </mrow><mrow>
  </mrow>
  </md>
  Substituting <m>t_1=2t_2</m> into the Method 1 equations gives the Method 2
  equations, and substituting <m>t_3=1-t_2</m> into the Method 3 equations gives
  the Method 2 equations. So all three really give the same line, just parametrized a little differently,
  </p>

  </example>

<warning xml:id="warn_line_normal">
  <title>A line in three dimensions has infinitely many normal vectors</title>
<p>For example, the line
  <me>
  \llt x-1,y-1,z\rgt=t\llt 1,2,-2\rgt
  </me>
  has direction vector <m>\llt 1,2,-2\rgt</m>. Any vector perpendicular to
  <m>\llt 1,2,-2\rgt </m>
  is perpendicular to the line. The vector <m>\llt n_1,n_2,n_3\rgt</m> is
  perpendicular to <m>\llt 1,2,-2\rgt</m> if and only if
  <me>
  0=\llt 1,2,-2\rgt \cdot \llt n_1,n_2,n_3\rgt = n_1+2n_2-2n_3
  </me>
  There is  whole plane of <m>\llt n_1,n_2,n_3\rgt</m>'s obeying this condition,
  of which <m>\llt 2,-1,0\rgt</m>, <m>\llt 0,1,1\rgt</m> and <m>\llt 2,0,1\rgt</m>
  are only three examples.
</p>

</warning>

<example xml:id="eg_VPdistance-point-line">
  <p>
  In this example, we find the distance between the point <m>(2,3,-1)</m> and the line
  <md>
  <mrow>
      L&amp;:\  \llt x-1,y-2,z-3\rgt=t\llt 1,1,2\rgt 
  </mrow><mrow>
      &amp;\quad \text{or, equivalently,}\quad
       x=1+t,\ y=2+t,\ z=3+2t
  </mrow> 
  </md>
  The vector from <m>(2,3,-1)</m> to the point <m>(1+t\,,\,2+t\,,\,3+2t)</m> on <m>L</m> is
  <m>
  \llt t-1\,,\,t-1\,,\,2t+4\rgt</m>.
  The square of the distance between <m>(2,3,-1)</m> and the point
  <m>(1+t\,,\,2+t\,,\,3+2t)</m>  on <m>L</m> is the square of the length of that vector, namely
  <me>
  d(t)^2 = (t-1)^2 +(t-1)^2 +(2t+4)^2
  </me>
  The point on <m>L</m> that is closest to <m>(2,3,-1)</m> is that whose value of <m>t</m>
  obeys
  <md>
  <mrow>
  0= \diff{}{t} d(t)^2 = 2(t-1) +2(t-1) + 2(2)(2t+4)
  \tag{\(*\)}</mrow>
  </md>
  </p>

  <p>Before we solve this equation for <m>t</m> and finish of our computation, observe
  that this equation (divided by <m>2</m>) says that
  <me>
  \llt 1\,,\,1\,,\,2\rgt\cdot\llt t-1\,,\,t-1\,,\, 2t+4\rgt = 0
  </me>
  That is, <em>the vector from <m>(2,3,-1)</m> to the point on <m>L</m> nearest <m>(2,3,-1)</m>
  is perpendicular to <m>L</m>'s direction vector</em>.
  </p>

  <p>Now back to our computation. The equation <m>(*)</m> simplifies to <m>12t+12=0</m>.
  So the optimal <m>t=-1</m> and the distance is
  <md>
  <mrow>
  d(-1) =\sqrt{(-1-1)^2+(-1-1)^2+(-2+4)^2}
  =\sqrt{12}
  </mrow>
  </md>
  </p>

</example>

<example xml:id="eg_VPdistance-point-line-bis">
  <title>Example <xref ref="eg_VPdistance-point-line"/> revisited</title>
  <p>
  In this example, we again find the distance between the point <m>(2,3,-1)</m>
  and the line
  <me>
  L:\  \llt x-1,y-2,z-3\rgt=t\llt 1,1,2\rgt
  </me>
  but we use a different method. In the figure below, <m>Q</m> is the point <m>(2,3,-1)</m>.
</p>
  <sidebyside width="45%">
  <image source="figs/pointDistProjB.svg"/>
  </sidebyside>
<p>
  If we drop a perpendicular from <m>Q</m> to the line <m>L</m>, it hits the line <m>L</m>
  at the point <m>N</m>, which is the point on <m>L</m> that is nearest <m>Q</m>. So
  the distance from <m>Q</m> to <m>L</m> is exactly the distance from <m>Q</m> to <m>N</m>, which
  is exactly the length of the vector from <m>Q</m> to <m>N</m>. In the figure above,
  <m>\vw</m> is the vector from <m>Q</m> to <m>N</m>. Now the vector <m>\vw</m> has to be perpendicular to the direction vector for <m>L</m>. That is,  <m>\vw</m> has to be perpendicular to <m>\vd=\llt 1,1,2\rgt</m>. However, as we saw in Warning
  <xref ref="warn_line_normal"/>, there are a huge number of vectors in different
  directions that are perpendicular to <m>\vd</m>. So you might think that it is very hard to even determine the direction of <m>\vw</m>.
  </p>

  <p>Fortunately, it isn't. Here is the strategy.
  <ul>
  <li>
  Pick any point on <m>L</m> and call it <m>P</m>.
  </li>
  <li>
  It is very easy to find the vector from <m>P</m> to <m>N</m> <mdash/> it is just the projection of the vector from <m>P</m> to <m>Q</m> (called <m>\vv</m> in the figure above)
  on <m>\vd</m>.
  </li>
  <li>
  Once we know <m>{\rm proj}_{\vd}\,\vv</m>, we will be able to compute
  <me>
  \vw = {\rm proj}_{\vd}\,\vv -\vv
  </me>
  </li>
  <li>
  and then the distance from <m>Q</m> to the line <m>L</m> is just <m>|\vw|</m>.
  </li>
  </ul>
</p>
<p>
  Here is the computation. We'll choose <m>P</m> to be the point on <m>L</m> that has
  <m>t=0</m>, which is <m>(1,2,3)</m>. So the vector from <m>P=(1,2,3)</m> to <m>Q=(2,3,-1)</m> is
  <me>
  \vv = \llt 2-1,3-2,-1-3\rgt=\llt 1,1,-4\rgt
  </me>
  The projection of <m>\vv=\llt 1,1,-4\rgt</m> on <m>\vd=\llt 1,1,2\rgt</m> is
  <me>
  {\rm proj}_{\vd}\,\vv
  =\frac{\llt 1,1,-4\rgt\cdot\llt 1,1,2\rgt}{|\llt 1,1,2\rgt|^2}\llt 1,1,2\rgt
  =\frac{-6}{6}\llt 1,1,2\rgt
  =\llt -1,-1,-2\rgt
  </me>
  and then
  <me>
  \vw = {\rm proj}_{\vd}\,\vv -\vv
      = \llt -1,-1,-2\rgt -\llt 1,1,-4\rgt
      = \llt -2,-2,2\rgt
  </me>
  and finally the distance from <m>Q</m> to the  line <m>L</m> is
  <me>
  |\vw| = |\llt -2,-2,2\rgt|
        =|2\llt -1,-1,1\rgt|
        =2\sqrt{3}
  </me>
  </p>
</example>

<example xml:id="eg_VPdistance-line-line"><title>(Optional) Distance between lines</title>
  <p>
  In this example, we find the distance between the lines
  <md>
  <mrow>
  L&amp;:\  \llt x-1,y-2,z-3\rgt = t \llt 1,0,-1 \rgt
  </mrow><mrow>
  L'&amp;:\ \llt x-1,y-2,z-1\rgt = t \llt 1,-2,1 \rgt
  </mrow>
  </md>
  We can rewrite the equations of the lines as
  <md>
  <mrow>
  L&amp;:\  x=1+t,\ y=2,\ z=3-t
  </mrow><mrow>
  L'&amp;:\ x=1+t,\ y=2-2t,\ z=1+t
  </mrow>
  </md>
  Of course the value of <m>t</m> in the parametric equation for <m>L</m> need not be
  the same as the value of <m>t</m> in the parametric equation for <m>L'</m>. So
  let us denote by <m>\vx(s) = (1+s\,,\,2\,,\,3-s)</m> and
  <m>\vy(t) = (1+t\,,\,2-2t\,,\,1+t)</m>
  the points on <m>L</m> and <m>L'</m>, respectively, that are closest together.
  Note that the vector from <m>\vx(s)</m> to <m>\vy(t)</m> is
  <m>\llt  t-s\,,\,-2t\,,\,-2+s+t \rgt</m>. Then, in particular,
  <ul>
  <li>
  <m>\vx(s)</m> is the point on <m>L</m> that is closest to the point <m>\vy(t)</m>, and
  </li>
  <li>
  <m>\vy(t)</m> is the point on <m>L'</m> that is closest to the point <m>\vx(s)</m>.
  </li>
  </ul>
  So, as we saw in Example <xref ref="eg_VPdistance-point-line"/>,
  the vector, <m>\llt  t-s\,,\,-2t\,,\,-2+s+t \rgt</m>, that joins <m>\vx(s)</m> and <m>\vy(t)</m>, must be perpendicular to both the direction vector of <m>L</m> and the
  direction vector of <m>L'</m>. Consequently
  <md alignment="alignat">
  <mrow>
  0&amp;= \llt 1,0,-1\rgt\cdot\llt  t-s\,,\,-2t\,,\,-2+s+t \rgt
   &amp;&amp;= \phantom{-}2-2s
 </mrow><mrow>
  0&amp;= \llt 1,-2,1\rgt\cdot\llt  t-s\,,\,-2t\,,\,-2+s+t \rgt
   &amp;&amp;=-2+6t
  </mrow>
  </md>
  So <m>s=1</m> and <m>t=\frac{1}{3}</m> and the distance between <m>L</m> and <m>L'</m> is
  <md>
  <mrow>
  \big|\llt  t-s\,,\,-2t\,,\,-2+s+t \rgt\big|_{s=1,\ t=1/3}
  &amp;=\big|\llt -2/3\,,\,-2/3\,,\,-2/3 \rgt\big|_{s=1,\ t=1/3}
  </mrow><mrow>
  &amp;=\frac{2}{\sqrt{3}}
  </mrow>
  </md>
  </p>

</example>


<example xml:id="eg_VPdistance-line-line-bis"><title>Example <xref ref="eg_VPdistance-line-line"/> revisited, again optional</title>
  <p>
  In this example, we again find the distance between the lines
  <md>
  <mrow>
  L&amp;:\  \llt x-1,y-2,z-3\rgt = t \llt 1,0,-1 \rgt
  </mrow><mrow>
  L'&amp;:\ \llt x-1,y-2,z-1\rgt = t \llt 1,-2,1 \rgt
  </mrow>
  </md>
  this time using a projection, much as in
  Example <xref ref="eg_VPdistance-point-plane-bis"/>. The procedure,
  which will be justified below, is
  <ul>
  <li>
  first form a vector <m>\vn</m> that is perpendicular to the direction vectors
  of both lines by taking the cross product of the two direction vectors.
  In this example,
  <md>
  <mrow>
  \llt 1,0,-1\rgt \times\llt 1,-2,1\rgt
      &amp; = \det\left[\begin{matrix}
        \hi&amp;\hj&amp;\hk \\ 1 &amp; 0 &amp; -1 \\ 1 &amp;-2 &amp; 1\end{matrix}\right]
      = -2\hi -2 \hj -2\hk
  </mrow>
  </md>
  Since we just want <m>\hn</m> to be perpendicular to both direction vectors,
  we may simplify our computations by dividing this vector by <m>-2</m>, and take
  <m>\vn = \llt 1,1,1 \rgt</m>.
  </li>
  <li>
  Next find one point on <m>L</m> and one point on <m>L'</m> and subtract to form a
  vector <m>\vv</m> whose tail is at one point and whose head is at the
  other point. This vector goes from one line to the other line. In this example,
  the point <m>(1,2,3)</m> is on <m>L</m> (just set <m>t=0</m> in the equation for <m>L</m>) and the point <m>(1,2,1)</m> is on <m>L'</m> (just set <m>t=0</m> in the equation for <m>L'</m>),
  so that we may take
  <me>
  \vv = \llt 1-1\,,\,2-2\,,\,3-1\rgt = \llt 0,0,2 \rgt
  </me>
  </li>
  <li>
  The distance between the two lines is the length of the projection of <m>\vv</m>
  on <m>\vn</m>. In this example, by <xref ref="eqn_proj"/>, the distance is
  <md>
  <mrow>
  \big|{\rm proj}_{\vn}\,\vv\big|
  &amp;=\left|\frac{\vv\cdot\vn}{|\vn|^2}\,\vn\right|
   =\frac{|\vv\cdot\vn|}{|\vn|}
  </mrow><mrow>
  &amp;= \frac{|\llt 0,0,2\rgt\cdot\llt 1,1,1\rgt|}{|\llt 1,1,1\rgt|}
  </mrow><mrow>
      &amp;= \frac{2}{\sqrt{3}}
  </mrow>
  </md>
  just as we found in Example <xref ref="eg_VPdistance-line-line"/>
  </li>
  </ul>
  Now, here is the justification for the procedure.
  <ul>
  <li>
  As we did in Example <xref ref="eg_VPdistance-line-line"/>, denote by
  <m>\vx(s)</m> and <m>\vy(t)</m> the points on <m>L</m> and <m>L'</m>, respectively,
  that are closest together. Note that, as we observed in
  Example <xref ref="eg_VPdistance-line-line"/>, the vector from <m>\vx(s)</m> to <m>\vy(t)</m>
  is perpendicular to the direction vectors of both lines, and so is parallel
  to <m>\vn</m>.
  </li>
  <li>
  Denote by <m>P</m> the plane through <m>\vx(s)</m> that is perpendicular to <m>\vn</m>.
  As <m>\vx(s)</m> is on <m>L</m> and the direction vector of <m>L</m> is perpendicular to
  <m>\vn</m>, the line <m>L</m> is contained in <m>P</m>.
  </li>
  <li>
  Denote by <m>P'</m> the plane through <m>\vy(t)</m> that is perpendicular to <m>\vn</m>.
  As <m>\vy(t)</m> is on <m>L'</m> and the direction vector of <m>L'</m> is perpendicular to
  <m>\vn</m>, the line <m>L'</m> is contained in <m>P'</m>.
  </li>
  <li>
  The planes <m>P</m> and <m>P'</m> are parallel to each other. As <m>\vx(s)</m> is on <m>P</m>
  and <m>\vy(t)</m> is on <m>P'</m>, and the vector from <m>\vx(s)</m> to <m>\vy(t)</m>
  is perpendicular to both <m>P</m> and <m>P'</m>, the distance from <m>P</m> to <m>P'</m>
  is exactly the length of the vector from <m>\vx(s)</m> to <m>\vy(t)</m>.
  That is also the distance from <m>L</m> to <m>L'</m>.
  </li>
  <li>
    <p>
  The vector <m>\vv</m> constructed in the procedure above is a vector between <m>L</m> and <m>L'</m> and so is also a vector between <m>P</m> and <m>P'</m>. Looking at the figure
  below
  <fn>and possibly reviewing the Definition <xref ref="def_projection"/>
  of projection</fn>,
  we see that the vector from <m>\vx(s)</m> to <m>\vy(t)</m> is
  (up to a sign) the projection of <m>\vv</m> on <m>\vn</m>.
  </p>

  <sidebyside width="55%">
  <image source="figs/planeDistB.svg"/>
  </sidebyside>
  </li>

  <li>
  So the distance from <m>P</m> to <m>P'</m>, and hence the distance from <m>L</m> to <m>L'</m>,
  is exactly the length of <m>{\rm proj}_{\vn}\vv</m>.
  </li>
  </ul>
  </p>

  </example>

  <xi:include href="../problems/prob_s1.5.ptx" />

</section>
