<?xml version="1.0" encoding="UTF-8" ?>
<section xmlns:xi="http://www.w3.org/2001/XInclude" xml:id="sec_surface_area">

<!-- Copyright 2018-2020 Joel Feldman, Andrew Rechnitzer and Elyse Yeager -->
<!-- This work is licensed under the Creative Commons Attribution-NonCommercial-ShareAlike 4.0 International License-->
<!-- https://creativecommons.org/licenses/by-nc-sa/4.0 -->

<title>Surface Area</title>
<p>
Suppose that we wish to find the area of part, <m>S</m>, of the surface <m>z=f(x,y)</m>. We start by cutting <m>S</m> up into tiny pieces. To do so,
<ul>
<li>
we draw a bunch of curves of constant <m>x</m> (the blue curves in the
figure below). Each such curve is the intersection of <m>S</m> with
the plane <m>x=x_0</m> for some constant <m>x_0</m>.  And we also
</li>
<li>
draw a bunch of curves of constant <m>y</m> (the red curves in the
figure below). Each such curve is the intersection of <m>S</m> with
the plane <m>y=y_0</m> for some constant <m>y_0</m>.
</li>
</ul>
</p>

<sidebyside>
<image source="problems/figs/sphericaldSxy.pdf"/>
</sidebyside>
<p>
Concentrate on any one the tiny pieces. Here is a greatly magnified
sketch of it, looking at it from above.
</p>

<sidebyside>
<image source="problems/figs/dSfxy.pdf"/>
</sidebyside>
<p>
We wish to compute its area, which we'll call <m>\dee{S}</m>.
Now this little piece of surface need not be parallel to the <m>xy</m>-plane,
and indeed need not even be flat. But if the piece is really tiny, it's
almost flat. We'll now approximate it by something that is flat,
and whose area we know. To start, we'll determine the corners of the piece.
To do so, we first determine the bounding curves of the piece.
Look at the figure above, and recall that, on the surface <m>z=f(x,y)</m>.
<ul>
<li>
The  upper blue curve was constructed by holding <m>x</m> fixed
at the value <m>x_0</m>, and sketching the curve swept out by
<m>x_0\,\hi+y\,\hj + f(x_0,y)\,\hk</m> as <m>y</m> varied, and
</li>
<li>
the  lower blue curve was constructed by holding <m>x</m> fixed
at the slightly larger value <m>x_0+\dee{x}</m>, and sketching the
curve swept out by  <m>(x_0+\dee{x})\,\hi+y\,\hj + f(x_0+\dee{x},y)\,\hk</m> as
<m>y</m> varied.
</li>
<li>
The red curves were constructed similarly, by holding <m>y</m> fixed
and varying <m>x</m>.
</li>
</ul>
So the four intersection points in the figure are
<md alignment="alignat">
<mrow>{3}
P_0&amp;=x_0\,\hi+y_0\,\hj + f(x_0,y_0)\,\hk
</mrow><mrow>
   P_1&amp;=x_0\,\hi+(y_0+\dee{y})\,\hj + f(x_0,y_0+\dee{y})\,\hk
</mrow><mrow>
P_2&amp;=(x_0+\dee{x})\,\hi+y_0\,\hj + f(x_0+\dee{x},y_0)\,\hk
</mrow><mrow>
   P_3&amp;=(x_0+\dee{x})\,\hi+(y_0+\dee{y})\,\hj + f(x_0+\dee{x},y_0+\dee{y})\,\hk
</mrow>
</md>
Now, for any small constants <m>\dee{X}</m> and <m>\dee{Y}</m>, we have the linear
approximation
<fn>Recall <xref ref="eqn_lin_approx_2d"/>.</fn>
<md>
<mrow>
f(x_0+\dee{X},y_0+\dee{Y})
&amp;\approx f(x_0\,,\,y_0)
   +\pdiff{f}{x}(x_0\,,\,y_0)\,\dee{X}
   +\pdiff{f}{y}(x_0\,,\,y_0)\,\dee{Y}
</mrow>
</md>
Applying this three times,
once with <m>\dee{X}=0</m>, <m>\dee{Y}=\dee{y}</m> (to approximate <m>P_1</m>),
once with <m>\dee{X}=\dee{x}</m>, <m>\dee{Y}=0</m> (to approximate <m>P_2</m>),
and once with  <m>\dee{X}=\dee{x}</m>, <m>\dee{Y}=\dee{y}</m> (to approximate <m>P_3</m>),
<md alignment="alignat">
<mrow>
P_1&amp;\approx P_0 \phantom{\ +\ \dee{x}\,\hi}
   \ +\ \dee{y}\,\hj\ \ +\   \pdiff{f}{y}(x_0\,,\,y_0)\,\dee{y}\,\hk
</mrow><mrow>
P_2&amp;\approx P_0
   \ +\ \dee{x}\,\hi  \phantom{\ +\  \dee{y}\,\hj}
   \ \ +\  \pdiff{f}{x}(x_0\,,\,y_0)\,\dee{x}\,\hk
</mrow><mrow>
P_3&amp;\approx P_0
   \ +\ \dee{x}\,\hi\ +\ \dee{y}\,\hj \ +\
           \Big[ \pdiff{f}{x}(x_0\,,\,y_0)\,\dee{x}
                               +  \pdiff{f}{y}(x_0\,,\,y_0)\,\dee{y}\Big]\,\hk
</mrow>
</md>
Of course we have only approximated the positions of the corners and
so have introduced errors. However, with more work, one can bound
those errors (like we in the optional ยง<xref ref="sec_integral_error"/>)
and show that in the limit <m>\dee{x},\dee{y}\rightarrow 0</m>, all of the
error terms that we dropped contribute exactly <m>0</m> to the integral.
</p>

<p>The small piece of our
surface with corners <m>P_0</m>, <m>P_1</m>, <m>P_2</m>, <m>P_3</m>  is approximately a parallelogram with sides
</p>

<sidebyside >
<p>
<md>
<mrow>
\overrightarrow{P_0P_1}
\approx \overrightarrow{P_2P_3}
&amp;\approx \dee{y}\,\hj\ +\   \pdiff{f}{y}(x_0\,,\,y_0)\,\dee{y}\,\hk
</mrow><mrow>
\overrightarrow{P_0P_2}
\approx \overrightarrow{P_1P_3}
&amp;\approx \dee{x}\,\hi\ +\  \pdiff{f}{x}(x_0\,,\,y_0)\,\dee{x}\,\hk
\qquad\qquad
</mrow>
</md>
</p>
<image source="problems/figs/dS2fxy.pdf"/>
</sidebyside>

<p>
Denote by <m>\theta</m> the angle between the vectors
<m>\overrightarrow{P_0P_1}</m> and <m>\overrightarrow{P_0P_2}</m>.
The base of the parallelogram, <m>\overrightarrow{P_0P_1}</m>,
has length <m>\big|\overrightarrow{P_0P_1}\big|</m>, and the height of the
parallelogram is <m>\big|\overrightarrow{P_0P_2}\big|\,\sin\theta</m>.
So the area of the parallelogram is
<fn>As we mentioned above,
the approximation below becomes exact when the limit <m>\dee{x}
,\dee{y}\rightarrow 0</m> is taken in the definition of the integral.
See ยง\eref{CLP317}{sec:hoterms} in the CLP-4 text.</fn>, by
Theorem <xref ref="thm_crossPppties"/>,
<md>
<mrow>
\dee{S}
=|\overrightarrow{P_0P_1}|\ |\overrightarrow{P_0P_2}| \ \sin\theta
&amp;= \big|\overrightarrow{P_0P_1}\times\overrightarrow{P_0P_2}\big|
</mrow><mrow>
&amp;\approx \bigg|\left(\hj\ +\   \pdiff{f}{y}(x_0\,,\,y_0)\,\hk\right)\times
              \left(\hi\ +\   \pdiff{f}{x}(x_0\,,\,y_0)\,\hk\right)\bigg|
          \dee{x}\dee{y}
</mrow>
</md>
The cross product is easily evaluated:
<md>
<mrow>
\left(\hj\ +\   \pdiff{f}{y}(x_0\,,\,y_0)\,\hk\right)\times
              \left(\hi\ +\   \pdiff{f}{x}(x_0\,,\,y_0)\,\hk\right)
&amp;=\det\left[\begin{matrix}
           \hi &amp; \hj &amp; \hk \\
           0 &amp; 1 &amp; \frac{\partial f}{\partial y}(x_0,y_0) \\
           1 &amp; 0 &amp; \frac{\partial f}{\partial x}(x_0,y_0)
           \end{matrix}\right]
</mrow><mrow>
&amp;= f_x(x_0,y_0)\,\hi + f_y(x_0,y_0)\,\hj - \hk
</mrow>
</md>
as is its length:
<md>
<mrow>
\left|\left(\hj\ +\   \pdiff{f}{y}(x_0\,,\,y_0)\,\hk\right)\times
              \left(\hi\ +\   \pdiff{f}{x}(x_0\,,\,y_0)\,\hk\right)\right|
&amp;= \sqrt{1 + f_x(x_0,y_0)^2 + f_y(x_0,y_0)^2}
</mrow>
</md>
Throughout this computation, <m>x_0</m> and <m>y_0</m> were arbitrary.
So we have found the area of each tiny piece of the surface <m>S</m>.
</p>


<fact xml:id="eq_dSgraph">
<statement>
<p>
For the surface <m>z=f(x,y)</m>,
<md>
<mrow>
\dee{S}&amp;= \sqrt{1 + f_x(x,y)^2 + f_y(x,y)^2}\
          \dee{x}\dee{y}
</mrow>
</md>
Similarly, for the surface <m>x=g(y,z)</m>,
<md>
<mrow>
\dee{S}&amp;= \sqrt{1 + g_y(y,z)^2 + g_z(y,z)^2}\
          \dee{y}\dee{z}
</mrow>
</md>
and for the surface <m>y=h(x,z)</m>,
<md>
<mrow>
\dee{S}&amp;= \sqrt{1 + h_x(x,z)^2 + h_z(x,z)^2}\
          \dee{x}\dee{z}
</mrow>
</md>
</p>
</statement>
</fact>

<p>
Consequently, we have
</p>


<theorem xml:id="thm_surface_area">
<statement><p>
<ol label="a">
<li>
The area of the part of the surface <m>z=f(x,y)</m> with <m>(x,y)</m> running over the
region <m>\cD</m> in the <m>xy</m>-plane is
<me>
\dblInt_\cD \sqrt{1 + f_x(x,y)^2 + f_y(x,y)^2}\
          \dee{x}\dee{y}
</me>
</li>
<li>
The area of the part of the surface <m>x=g(y,z)</m> with <m>(y,z)</m> running over the
region <m>\cD</m> in the <m>yz</m>-plane is
<me>
\dblInt_\cD \sqrt{1 + g_y(y,z)^2 + g_z(y,z)^2}\
          \dee{y}\dee{z}
</me>
</li>
<li>
The area of the part of the surface <m>y=h(x,z)</m> with <m>(x,z)</m> running over the
region <m>\cD</m> in the <m>xz</m>-plane is
<me>
\dblInt_\cD \sqrt{1 + h_x(x,z)^2 + h_z(x,z)^2}\
          \dee{x}\dee{z}
</me>
</li>
</ol>
</p></statement>
</theorem>

<!--
\intremark{
The formulae like
<m>\dee{S}= \sqrt{1 + f_x(x,y)^2 + f_y(x,y)^2}\ \dee{x}\dee{y}</m>
in <xref ref="eq_dSgraph"/> have geometric interpretations. The red
parallelogram in the sketch
</p>

<sidebyside>
<image source="problems/figs/surfaceProj.pdf"/>
</sidebyside>
represents a little piece of our surface. It has area
<m>\dee{S}= \sqrt{1 + f_x(x,y)^2 + f_y(x,y)^2}\ \dee{x}\dee{y}</m>.
The blue parallelogram in the same sketch represents the projection
of the red parallelogram onto the <m>xy</m>-plane. It has area <m>\dee{x}\dee{y}</m>.
The vector <m>\hn</m> in the sketch is a unit normal for the red parallelogram.
We have seen that it is parallel to
<me>
\frac{\partial\vr}{\partial x}\times
              \frac{\partial\vr}{\partial y}
= -f_x(x,y)\,\hi - f_y(x,y)\,\hj + \hk
</me>
so that the angle <m>\theta</m> between <m>\hn</m> and <m>\hk</m> obeys
<md>
<mrow>
\cos\theta &amp;= \frac{(-f_x(x,y)\,\hi - f_y(x,y)\,\hj + \hk)\cdot\hk}
                 {\big|-f_x(x,y)\,\hi - f_y(x,y)\,\hj + \hk\big|\,|\hk|}
</mrow><mrow>
&amp;=\frac{1}{\sqrt{1 + f_x(x,y)^2 + f_y(x,y)^2}}
</mrow>
</md>
The geometric interpretation of
<m>\dee{S}= \sqrt{1 + f_x(x,y)^2 + f_y(x,y)^2}\ \dee{x}\dee{y}</m>
is that the area <m>\dee{S}</m> of a little piece of surface is the
area of its projection on the <m>xy</m>-plane times the factor
<m>\frac{1}{\cos\theta}</m> where <m>\theta</m> is the angle between <m>\hn</m>
(which is perpendicular to the surface) and <m>\hk</m> (which is
perpendicular to the <m>xy</m>-plane). Notice that
<ul>
<li>sep1pt \parskip0pt \parsep0pt
</li>
<li>[<m>\circ</m>]
when <m>\theta</m> is close to zero, which corresponds the <m>f</m> being almost constant
and our surface being almost parallel to the <m>xy</m>-plane, <m>\dee{S}</m>
reduces to almost <m>\dee{x}\dee{y}</m>.
</li>
<li>[<m>\circ</m>]
On the other hand, in the limit <m>\theta\rightarrow\frac{\pi}{2}</m>, which
corresponds to <m>f_x</m> and/or <m>f_y</m> becoming infinite
and our surface becoming perpendicular to the <m>xy</m>-plane,
<m>\dee{S}</m> becomes <q>infinity times</q> <m>\dee{x}\dee{y}</m>. In this case,
we should represent our surface either in the form <m>x=g(y,z)</m>
or in the form <m>y=h(x,z)</m>, rather than in the form <m>z=f(x,y)</m>.
</li>
</ul>
}
 -->

<example xml:id="eg_area_cone"><title>Area of a cone</title>
<p>
As a first example, we compute the area of the part of the
cone
<me>
z=\sqrt{x^2+y^2}
</me>
with <m>0\le z\le a</m> or, equivalently, with <m>x^2+y^2\le a^2</m>.
</p>

<sidebyside>
<image source="problems/figs/cone"/>
</sidebyside>
<p>
Note that <m>z=\sqrt{x^2+y^2}</m> is the side of the cone. It does not include the top.
</p>

<p>To find its area, we will apply <xref ref="eq_dSgraph"/> to
<me>
z=f(x,y) = \sqrt{x^2+y^2}
\qquad\text{with $(x,y)$ running over } x^2+y^2\le a^2
</me>
That forces us to compute the first order partial derivatives
<md>
<mrow>
f_x(x,y) &amp; = \frac{x}{\sqrt{x^2+y^2}}
</mrow><mrow>
f_y(x,y) &amp; = \frac{y}{\sqrt{x^2+y^2}}
</mrow><mrow>
</mrow>
</md>
Substituting them into the first formula in <xref ref="eq_dSgraph"/> yields
<md>
<mrow>
\dee{S}&amp;= \sqrt{1 + f_x(x,y)^2 + f_y(x,y)^2}\  \dee{x}\,\dee{y}
</mrow><mrow>
   &amp;=\sqrt{1+\Big(\frac{x}{\sqrt{x^2+y^2}}\Big)^2
            +\Big(\frac{y}{\sqrt{x^2+y^2}}\Big)^2} \ \dee{x}\,\dee{y}
</mrow><mrow>
   &amp;=\sqrt{1+\frac{x^2+y^2}{x^2+y^2}} \ \dee{x}\,\dee{y}
</mrow><mrow>
   &amp;=\sqrt{2} \ \dee{x}\,\dee{y}
</mrow>
</md>
So
<md>
<mrow>
\text{Area}
&amp;= \dblInt_{x^2+y^2\le a^2} \sqrt{2}\ \dee{x}\,\dee{y}
= \sqrt{2} \dblInt_{x^2+y^2\le a^2} \dee{x}\,\dee{y}
= \sqrt{2} \pi a^2
</mrow>
</md>
because <m>\dblInt_{x^2+y^2\le a^2} \dee{x}\,\dee{y}</m> is exactly
the area of a circular disk of radius <m>a</m>.
</p></example>

<example xml:id="eg_area_cylinder"><title>Area of a cylinder</title>
<statement>
<p>
Let <m>a,b \gt 0</m>. Find the surface area of
<me>
\cS = \Set{(x,y,z)}{x^2+z^2=a^2,\ 0\le y\le b}
</me>
</p>
</statement>

<solution>
<p>
The intersection of <m>x^2+z^2=a^2</m> with any plane of constant <m>y</m>
is the circle of radius <m>a</m> centred on <m>x=z=0</m>. So <m>\cS</m> is a
bunch of circles stacked sideways. It is a cylinder on its side (with both
ends open).
By symmetry, the area of <m>\cS</m> is four times the area of the part of <m>\cS</m>
that is in the first octanct, which is
<me>
\cS_1 = \Big\{(x,y,z)\ \Big|\ z=f(x,y)=\sqrt{a^2-x^2},\ 0\le x\le a,\
                               0\le y\le b\Big\}
</me>
</p>

<sidebyside>
<image source="problems/figs/cylinderF.pdf"/>
<image source="problems/figs/cylinderG.pdf"/>
</sidebyside>

<p>
Since
<me>
f_x(x,y)=-\frac{x}{\sqrt{a^2-x^2}}\qquad
f_y(x,y)=0
</me>
the first formula in <xref ref="eq_dSgraph"/> yields
<md>
<mrow>
\dee{S}&amp;= \sqrt{1 + f_x(x,y)^2 + f_y(x,y)^2}\  \dee{x}\,\dee{y}
</mrow><mrow>
   &amp;=\sqrt{1+\Big(-\frac{x}{\sqrt{a^2-x^2}}\Big)^2} \ \dee{x}\,\dee{y}
</mrow><mrow>
   &amp;=\sqrt{1+\frac{x^2}{a^2-x^2}} \ \dee{x}\dee{y}
</mrow><mrow>
   &amp;=\frac{a}{\sqrt{a^2-x^2}} \ \dee{x}\dee{y}
</mrow>
</md>
So
<md>
<mrow>
\text{Area}(\cS_1)
&amp;= \int_0^a\dee{x}\int_0^b\dee{y}\ \frac{a}{\sqrt{a^2-x^2}}
=ab \int_0^a\dee{x} \frac{1}{\sqrt{a^2-x^2}}
</mrow>
</md>
The indefinite integral of <m>\frac{1}{\sqrt{a^2-x^2}}</m>
is <m>\arcsin\frac{x}{a}+C</m>. (See the table of integrals in Appendix
<xref ref="app_integral"/>. Alternatively, use the trig substitution <m>x=a\sin\theta</m>.)
So
<md>
<mrow>
\text{Area}(\cS_1)
= ab\left[\arcsin\frac{x}{a}\right]_0^a
= ab\big[\arcsin 1 -\arcsin 0\big]
=\frac{\pi}{2} ab
</mrow>
</md>
and
<md>
<mrow>
\text{Area}(\cS)
=4\text{Area}(\cS_1)
=2\pi ab
</mrow>
</md>
</p>

<p>We could have also come to this conclusion by using a little geometry,
rather than using calculus. Cut open the cylinder by cutting
along a line parallel to the <m>y</m>-axis, and then flatten out the
cylinder. This gives a rectangle. One side of the rectangle is just
a circle of radius <m>a</m>, straightened out. So the rectangle has sides
of lengths <m>2\pi a</m> and <m>b</m> and has area <m>2\pi ab</m>.
</p>
</solution>
</example>

<example xml:id="eg_area_hemisphere"><title>Area of a hemisphere</title>
<p>
This time we compute the surface area of the hemisphere
<me>
x^2+y^2+z^2=a^2\qquad z\ge 0
</me>
(with <m>a \gt 0</m>).
You probably know, from high school, that the answer is
<m>\frac{1}{2}\times 4\pi a^2=2\pi a^2</m>. But you have probably
not seen a derivation
<fn>There is a pun hidden here, because
you can (with a little thought) also get the surface area by differentiating
the volume with respect to the radius.</fn>
 of this answer.
Note that, since <m>x^2+y^2 = a^2-z^2</m> on the hemisphere, the set
of <m>(x,y)</m>'s for which there is a <m>z</m> with <m>(x,y,z)</m> on the  hemisphere
is exactly <m>\Set{(x,y)\in\bbbr^2}{x^2+y^2\le a^2}</m>.
So the hemisphere is
<md>
<mrow>
S &amp;= \Big\{(x,y,z)\ \Big|\ z=\sqrt{a^2-x^2-y^2},\ x^2+y^2\le a^2\Big\}
</mrow>
</md>
We will compute the area of <m>S</m> by applying <xref ref="eq_dSgraph"/> to
<me>
z=f(x,y) = \sqrt{a^2-x^2-y^2}
\qquad\text{with $(x,y)$ running over } x^2+y^2\le a^2
</me>
The first formula in <xref ref="eq_dSgraph"/> yields
<md>
<mrow>
\dee{S}&amp;= \sqrt{1 + f_x(x,y)^2 + f_y(x,y)^2}\  \dee{x}\dee{y}
</mrow><mrow>
   &amp;=\sqrt{1+\Big(\frac{-x}{\sqrt{a^2-x^2-y^2}}\Big)^2
            +\Big(\frac{-y}{\sqrt{a^2-x^2-y^2}}\Big)^2} \ \dee{x}\dee{y}
</mrow><mrow>
   &amp;=\sqrt{1+\frac{x^2+y^2}{a^2-x^2-y^2}} \ \dee{x}\dee{y}
</mrow><mrow>
   &amp;=\sqrt{\frac{a^2}{a^2-x^2-y^2}} \ \dee{x}\dee{y}
</mrow>
</md>
So the area is
<m>
\dblInt_{x^2+y^2\le a^2}\frac{a}{\sqrt{a^2-x^2-y^2}}
            \ \dee{x}\dee{y}
</m>.
To evaluate this integral, we switch to polar coordinates, substituting
<m>x=r\cos\theta</m>, <m>y=r\sin\theta</m>. This gives
<md>
<mrow>
\text{area}
&amp;=\dblInt_{x^2+y^2\le a^2}\frac{a}{\sqrt{a^2-x^2-y^2}}
            \ \dee{x}\dee{y}
=\int_0^a\dee{r}\ r\int_0^{2\pi}\dee{\theta}\  \frac{a}{\sqrt{a^2-r^2}}
</mrow><mrow>
&amp;=2\pi a \int_0^a\dee{r}\ \frac{r}{\sqrt{a^2-r^2}}
</mrow><mrow>
&amp;=2\pi a\int_{a^2}^0 \frac{-\dee{u}/2}{\sqrt{u}}
\qquad\text{with } u=a^2-r^2,\ \dee{u} = -2r\,\dee{r}
</mrow><mrow>
&amp;=2\pi a\Big[-\sqrt{u}\Big]_{a^2}^0
</mrow><mrow>
&amp;=2\pi a^2
</mrow>
</md>
as it should be.
</p>

</example>

<example xml:id="eg_area_paraboloid">
<statement>
<p>
Find the surface area of the part of the paraboloid <m>z=2-x^2-y^2</m>
lying above the <m>xy</m>-plane.
</p>
</statement>

<solution>
<p>
The equation of the surface is of the form <m>x=f(x,y)</m> with <m>f(x,y)=2-x^2-y^2</m>.
So
<md>
<mrow>
f_x(x,y) =-2x\qquad
f_y(x,y) =-2y
</mrow>
</md>
and, by the first part of <xref ref="eq_dSgraph"/>,
<md>
<mrow>
\dee{S} &amp;= \sqrt{1 + f_x(x,y)^2 + f_y(x,y)^2}\  \dee{x}\dee{y}
</mrow><mrow>
   &amp;=\sqrt{1+4x^2+4y^2} \ \dee{x}\dee{y}
</mrow>
</md>
The point <m>(x,y,z)</m>, with <m>z=2-x^2-y^2</m>, lies above the <m>xy</m>-plane if and only
if <m>z\ge 0</m>, or, equivalently, <m>2-x^2-y^2\ge 0</m>. So the domain of
integration is <m>\Set{(x,y)}{x^2+y^2\le 2}</m> and
<me>
\text{Surface Area} = \dblInt_{x^2+y^2\le 2}\ \sqrt{1+4x^2+4y^2} \ \dee{x}\dee{y}
</me>
Switching to polar coordinates,
<md>
<mrow>
\text{Surface Area}
&amp;=\int_0^{2\pi}\int_0^{\sqrt{2}}\sqrt{1+4r^2}\  r\,\dee{r}\, \dee{\theta}
</mrow><mrow>
&amp;=2\pi\left[\frac{1}{12}{\big(1+4r^2\big)}^{3/2}\right]_0^{\sqrt{2}}
=\frac{\pi}{6}[27-1]
</mrow><mrow>
&amp;=\frac{13}{3}\pi
</mrow>
</md>
</p>
</solution>
</example>

</section>
