<?xml version="1.0" encoding="UTF-8" ?>
<section xmlns:xi="http://www.w3.org/2001/XInclude" xml:id="sec_directional_derivatives">

<!-- Copyright 2018-2020 Joel Feldman, Andrew Rechnitzer and Elyse Yeager -->
<!-- This work is licensed under the Creative Commons Attribution-NonCommercial-ShareAlike 4.0 International License-->
<!-- https://creativecommons.org/licenses/by-nc-sa/4.0 -->

<title>Directional Derivatives and the Gradient</title>

<subsection><title>Directional Derivatives and the Gradient</title>
<introduction>
<p>The principal interpretation of <m>\diff{f}{x}(a)</m> is the rate of change of
<m>f(x)</m>, per unit change of <m>x</m>, at <m>x=a</m>. The natural analog of this
interpretation for multivariable functions is the directional derivative,
which we now introduce through a question.
</p>
</introduction>
<subsubsection><title>A Question</title>
<p>
Suppose that you are standing at <m>(a,b)</m> near a campfire.
The temperature you feel at <m>(x,y)</m> is <m>f(x,y)</m>. You start
to move with velocity <m>\vv=\llt v_1,v_2\rgt </m>. What rate of change of temperature do you feel?
</p>
</subsubsection>

<subsubsection><title>The Answer</title>
<p>
Let's set the beginning of time, <m>t=0</m>, to the time at which you leave
<m>(a,b)</m>. Then
<ul>
<li>
at time <m>0</m> you are at <m>(a, b)</m> and feel the
temperature <m>f(a, b)</m> and
</li>
<li>
at time <m>t</m> you are at <m>(a+v_1t\,,\, b+v_2t)</m> and feel the
temperature <m>f(a+v_1t\,,\, b+v_2t)</m>.  So
</li>
<li>
the change in temperature between time <m>0</m> and time <m>t</m> is
<m>f(a+v_1t\,,\, b+v_2t)-f(a,b)</m>,
</li>
<li>
the average rate of change of temperature, per unit time, between
time <m>0</m> and time <m>t</m> is <m>\frac{f(a+v_1t\,,\, b+v_2t)-f(a,b)}{t}</m> and the
</li>
<li>
instantaneous rate of change of temperature per unit time as you leave
<m>(a,b)</m> is
<m>
\lim\limits_{t\rightarrow 0}\frac{f(a+v_1t\,,\, b+v_2t)-f(a,b)}{t}
</m>.
</li>
</ul>
Concentrate on the <m>t</m> dependence in this limit by
writing <m>f(a+v_1t\,,\, b+v_2t)=g(t)</m>.  Then
<md>
<mrow>
\lim_{t\rightarrow 0}\frac{f(a+v_1t\,,\, b+v_2t)-f(a,b)}{t}
&amp;=\lim_{t\rightarrow 0}\frac{g(t)-g(0)}{t}
</mrow><mrow>
&amp;=\diff{g}{t}(0)
</mrow><mrow>
&amp;=\diff{}{t}\big[f(a+v_1t\,,\, b+v_2t)\big]\Big|_{t=0}
</mrow>
</md>
By the chain rule, we can write the right hand side in terms of
partial derivatives of <m>f</m>.
<me>
\diff{}{t}\big[f(a+v_1t\,,\, b+v_2t)\big]
  =f_x(a+v_1t\,,\, b+v_2t)\,v_1 + f_y(a+v_1t\,,\, b+v_2t)\,v_2
</me>
So, setting <m>t=0</m>,
<md>
<mrow>
&amp;\lim_{t\rightarrow 0}\frac{f(a+v_1t\,,\, b+v_2t)-f(a,b)}{t}
</mrow><mrow>
&amp;\hskip0.5in=\big[f_x(a+v_1t\,,\, b+v_2t)\,v_1 + f_y(a+v_1t\,,\, b+v_2t)\,v_2
                           \big]\Big|_{t=0}
</mrow><mrow>
&amp;\hskip0.5in=f_x(a,b)\,v_1+f_y(a,b)\,v_2
</mrow><mrow>
&amp;\hskip0.5in=\llt f_x(a,b)\,,\,f_y(a,b)\rgt \cdot\llt v_1,v_2\rgt
</mrow>
</md>
Notice that we have expressed the rate of change as the dot product
of the velocity vector with a vector of partial derivatives of <m>f</m>.
We have seen such a vector of partial derivatives of <m>f</m> before;
in Definition <xref ref="def_gradient"/>, we defined the
gradient of the three variable function <m>G(x,y,z)</m> at the point
<m>\big( x_0\,,\,y_0\,,\,z_0\big)</m> to be
<m>
\llt G_x\big( x_0\,,\,y_0\,,\,z_0\big)\,,\,
     G_y\big( x_0\,,\,y_0\,,\,z_0\big)\,,\,
     G_z\big( x_0\,,\,y_0\,,\,z_0\big)\rgt
</m>.
Here we see the natural two dimensional analog.
</p>

<definition xml:id="def_gradient_2d">
<statement><p>
The vector <m>\llt f_x(a,b)\,,\,f_y(a,b)\rgt </m> is denoted <m>\vnabla f(a,b)</m> and is
called <q>the <alert>gradient</alert> of the function <m>f</m> at the point <m>(a,b)</m></q>.
</p></statement>
</definition>

<p>
In general, the gradient of <m>f</m> is a vector with one component
for each variable of <m>f</m>. The <m>j^{\rm th}</m> component is the partial
derivative of <m>f</m> with respect to the <m>j^{\rm th}</m> variable.
</p>

<p>Now because the dot product <m>\vnabla f(a,b)\cdot\vv</m> appears frequently,
we introduce some handy notation.
</p>

<definition xml:id="def_dir_deriv">
<statement><p>
Given any vector <m>\vv=\llt v_1,v_2\rgt</m>,
the expression
<me>
\llt f_x(a,b),f_y(a,b)\rgt \cdot\llt v_1,v_2\rgt  =\vnabla f(a,b)\cdot\vv
</me>
is denoted <m>D_{\vv}f(a,b)</m>.
</p></statement>
</definition>

<p>
Armed with this useful notation we can answer our question very succinctly.
</p>

<fact xml:id="eqn_dir_deriv_time">
  <statement>
    <p>
The rate of change of <m>f</m> per unit
time as you leave <m>(a,b)</m> moving with velocity <m>\vv</m> is
<me>
D_{\vv}f(a,b)=\vnabla f(a,b)\cdot\vv
</me>
</p>
</statement>
</fact>

<p>We can compute the rate of change of temperature per unit distance
(as opposed to per unit time) in a similar way.  The change in
temperature between
time <m>0</m> and time <m>t</m> is <m>f(a+v_1t, b+v_2t)-f(a,b)</m>.
Between time <m>0</m> and time <m>t</m>, you have travelled a distance <m>|\vv|t</m>.
So the instantaneous rate of change of temperature per unit distance as you
leave <m>(a,b)</m> is
<md>
<mrow>
\lim_{t\rightarrow 0}\frac{f(a+v_1t, b+v_2t)-f(a,b)}{t|\vv|}
</mrow>
</md>
This is exactly <m>\frac{1}{|\vv|}</m> times
<m>\lim\limits_{t\rightarrow 0}\frac{f(a+v_1t, b+v_2t)-f(a,b)}{t}</m>
which we computed above to be <m>D_{\vv}f(a,b)</m>. So
</p>

<fact xml:id="eqn_dir_deriv_space">
  <statement>
    <p>
Given any nonzero vector <m>\vv</m>, the rate of change of <m>f</m> per unit
distance as you leave <m>(a,b)</m> moving in direction <m>\vv</m> is
<me>
\vnabla f(a,b)\cdot\frac{\vv}{|\vv|}
       =D_{\frac{\vv}{|\vv|}}\ f(a,b)
</me>
</p>
</statement>
</fact>

<definition xml:id="def_dri_deriv">
<statement><p>
<m>D_{\frac{\vv}{|\vv|}}\ f(a,b)</m> is called the <em>directional derivative</em>
of the function <m>f(x,y)</m> at the point <m>(a,b)</m> in the
direction
<fn>Some people require direction vectors to have unit
length. We don't. </fn>
 <m>\vv</m>.
</p></statement>
</definition>
</subsubsection>

<subsubsection><title>The Implications</title>
<p>
We have just seen that the instantaneous rate of change of <m>f</m> per unit
distance as we leave <m>(a,b)</m> moving in direction <m>\vv</m> is a dot product,
which we can write as
<me>
\vnabla f(a,b)\cdot\frac{\vv}{|\vv|}
       =|\vnabla f(a,b)| \cos \theta
</me>
where <m>\theta</m> is the angle between the gradient vector <m>\vnabla f(a,b)</m>
and the direction vector <m>\vv</m>. Writing it in this way allows us to make
some useful observations.
Since <m>\cos \theta</m> is always between <m>-1</m>
and <m>+1</m>
<ul>
<li>
the direction of maximum rate of increase is that having
<m>\theta=0</m>. So to get maximum rate of increase per unit distance, as you
leave <m>(a,b)</m>, you should move in the same direction as the gradient
<m>\vnabla f(a,b)</m>. Then the rate of increase per unit distance is
<m>|\vnabla f(a,b)|</m>.
</li>
<li>
The direction of minimum (i.e. most negative) rate of increase  is that having
<m>\theta=180^\circ</m>. To get minimum rate of increase per unit distance you
should move in the direction opposite  <m>\vnabla f(a,b)</m>. Then the
rate of increase per unit distance is <m>-|\vnabla f(a,b)|</m>.
</li>
<li>
The directions giving zero rate of increase are those
perpendicular to <m>\vnabla f(a,b)</m>. If you move in a direction
perpendicular to <m>\vnabla f(a,b)</m>, then <m>f(x,y)</m> remains constant as
you leave <m>(a,b)</m>. At that instant, you are moving so that <m>f(x,y)</m>
remains constant and consequently you are moving along the level
curve <m>f(x,y)=f(a,b)</m>.  So <m>\vnabla f(a,b)</m> is perpendicular to the
level curve <m>f(x,y)=f(a,b)</m> at <m>(a,b)</m>. The corresponding statement
in three dimensions is that <m>\vnabla F(a,b,c)</m> is perpendicular to the
level surface <m>F(x,y,z)=F(a,b,c)</m> at <m>(a,b,c)</m>. Hence a good way to find a
vector normal to the surface <m>F(x,y,z)=0</m> at the point <m>(a,b,c</m>) is to compute the gradient <m>\vnabla F(a,b,c)</m>. This is precisely what we saw back in
Theorem <xref ref="thm_tan_plane_G"/>.
</li>
</ul>
</p>

<p>Now that we have defined the directional derivative, here are some examples.
</p>

<example xml:id="eg_dir_deriv_A">
<statement>
<p>
Find the directional derivative of the function <m>f(x,y)=e^{x+y^2}</m>
at the point <m>(0,1)</m> in the direction <m>-\hi + \hj</m>.
</p>
</statement>

<solution>
<p>
To compute the directional derivative, we need the gradient.
To compute the gradient, we need some partial derivatives.
So we start with the partial derivatives of <m>f</m> at <m>(0,1)</m>:
<md alignment="alignat">
<mrow>
f_x(0,1) &amp;= e^{x+y^2}\Big|_{x=0\atop y=1} &amp;&amp;=e
</mrow><mrow>
f_y(0,1) &amp;= 2ye^{x+y^2}\Big|_{x=0\atop y=1} &amp;&amp;=2e
</mrow>
</md>
So the gradient of <m>f</m> at <m>(0,1)</m> is
<me>
\vnabla f(0,1) = f_x(0,1)\,\hi + f_y(0,1)\,\hj
               = e\,\hi + 2e\,\hj
</me>
and the direction derivative in the direction <m>-\hi + \hj</m> is
<me>
D_{\frac{-\hi+\hj}{|-\hi+\hj|}} f(0,1)
   = \vnabla f(0,1)\cdot\frac{-\hi+\hj}{|-\hi+\hj|}
   = \big(e\,\hi + 2e\,\hj\big)\cdot \frac{-\hi+\hj}{\sqrt{2}}
   = \frac{e}{\sqrt{2}}
</me>
</p>
</solution>
</example>

<example xml:id="eg_dir_deriv_B">
  <statement>
<p>
Find the directional derivative of the function <m>w(x,y,z)=xyz +\ln(xz)</m>
at the point <m>(1,3,1)</m> in the direction <m>\llt 1\,,\,0\,,\,1\rgt</m>.
In what directions is the directional derivative zero?
</p>
</statement>

<solution>
<p>
First, the partial derivatives of <m>w</m> at <m>(1,3,1)</m> are
<md alignment="alignat">
<mrow>
w_x(1,3,1) &amp;= \left[yz+\frac{1}{x}\right]\bigg|_{(1,3,1)}
             &amp;&amp;=3\times 1+\frac{1}{1}&amp;&amp;=4
</mrow><mrow>
w_y(1,3,1) &amp;= xz\bigg|_{(1,3,1)} &amp;&amp;=1\times 1&amp;&amp;=1
</mrow><mrow>
w_z(1,3,1) &amp;= \left[xy+\frac{1}{z}\right]\bigg|_{(1,3,1)} &amp;&amp;=1\times 3 +\frac{1}{1} &amp;&amp;=4
</mrow>
</md>
so the gradient of <m>w</m> at <m>(1,3,1)</m> is
<me>
\vnabla w(1,3,1) = \llt w_x(1,3,1)\,,\,w_y(1,3,1)\,,\,w_z(1,3,1)\rgt
               = \llt 4\,,\,1\,,\,4\rgt
</me>
and the direction derivative in the direction <m>\llt 1\,,\,0\,,\,1\rgt</m> is
<md>
<mrow>
D_{\frac{\llt 1\,,\,0\,,\,1\rgt}{|\llt 1\,,\,0\,,\,1\rgt|}} w(1,3,1)
   &amp;= \vnabla w(1,3,1)\cdot
              \frac{\llt 1\,,\,0\,,\,1\rgt}{|\llt 1\,,\,0\,,\,1\rgt|}
   = \llt 4\,,\,1\,,\,4\rgt\cdot \frac{\llt 1\,,\,0\,,\,1\rgt}{\sqrt{2}}
</mrow><mrow>
  &amp;= \frac{8}{\sqrt{2}}=4\sqrt{2}
</mrow>
</md>
The directional derivative of <m>w</m> at <m>(1,3,1)</m> in the direction <m>\vt\ne\vZero</m>
is zero if and only if
<me>
0 = D_{\frac{\vt}{|\vt|}} w(1,3,1)
   = \vnabla w(1,3,1)\cdot\frac{\vt}{|\vt|}
   = \llt 4\,,\,1\,,\,4\rgt\cdot \frac{\vt}{|\vt|}
</me>
which is the case if and only if <m>\vt</m> is perpendicular to
<m>\llt 4\,,\,1\,,\,4\rgt</m>. So if we walk in the direction of any vector
in the plane, <m>4x+y+4z=0</m> (which has normal vector <m>\llt 4\,,\,1\,,\,4\rgt</m>)
then the directional derivative is zero.
</p>
</solution>
</example>

<example xml:id="eg_dir_deriv_C">
<p>
Let
<me>
f(x,y)=5-x^2-2y^2\qquad
(a,b)=\big(-1,-1\big)
</me>
In this example, we'll explore the behaviour of the function <m>f(x,y)</m>
near the point <m>(a,b)</m>.
</p>

<p>Note that for any fixed <m>f_0 \lt 5</m>, <m>f(x,y)=f_0</m> is the ellipse
<m>x^2+2y^2=5-f_0</m>. So the graph <m>z=f(x,y)</m>
consists of a bunch of horizontal ellipses stacked one on top of
each other.
<ul>
<li><p>
Since the  ellipse <m>x^2+2y^2=5-f_0</m>  has <m>x</m>-semi-axis <m>\sqrt{5-f_0}</m>
and <m>y</m>-semi-axis <m>\sqrt{\frac{5-f_0}{2}}</m>,
<ul>
<li>
    the ellipses start with a point on the <m>z</m> axis when <m>f_0=5</m> and
</li>
<li>
    increase in size as <m>f_0</m> decreases.
</li>
</ul></p>
</li>
<li>
The part of the graph <m>z=f(x,y)</m> in the first octant is sketched in
the left hand figure below.
</li>
<li>
Several level curves, <m>f(x,y)=f_0</m>, are sketched in the right hand figure below.
</li>
<li>
The gradient vector
<me>
\vnabla f(a,b)=\llt -2x,-4y\rgt \big|_{(-1,-1)}=\llt 2,4\rgt
     =2\llt 1,2\rgt
</me>
at <m>(-1,-1)</m> is also illustrated in the righ hand sketch.
</li>
</ul>
We have that, at <m>(a,b)=(-1,-1)</m>,
<ul>
<li>
the unit vector giving the direction of maximum rate of increase is
the unit vector in the direction of the gradient vector <m>2\llt 1,2\rgt</m>,
which is <m>\frac{1}{\sqrt{5}}\llt 1,2\rgt</m>.
The maximum rate of  increase is  <m>|\llt 2,4\rgt |=2\sqrt{5}</m>.
</li>
<li>
The unit vector giving the direction of minimum rate of increase is
<m>-\frac{1}{\sqrt{5}}\llt 1,2\rgt </m> and that minimum rate is
<m>-|\llt 2,4\rgt |=-2\sqrt{5}</m>.
</li>
<li><p>
The directions giving zero rate of increase are perpendicular
to <m>\vnabla f(a,b)</m>. One vector perpendicular
<fn>
  Check this by taking the dot product of <m>\llt 1,2\rgt</m> and <m>\llt 2,-1\rgt</m>.
</fn>
to <m>\llt 1,2\rgt</m> is <m>\llt 2,-1\rgt</m>.  So the unit vectors giving the
direction of zero rate of increase are the  <m>\pm\frac{1}{\sqrt{5}}(2,-1)</m>.
These are the directions of the tangent vector at <m>(a,b)</m> to the level
curve of <m>f</m> through <m>(a,b)</m>, which is the curve <m>f(x,y)=f(a,b)</m>.
</p></li>
</ul>
</p>

<sidebyside widths="30% 50%" valign="middle">
<image source="figs/dderivB"/>
<image source="figs/dderivC"/>
</sidebyside>

</example>

<example xml:id="eg_dir_deriv_D">
<statement>
<p>
What is the rate of change of <m>f(x,y,z)=x^2+y^2+z^2</m> at <m>(3,5,4)</m> moving
in the positive <m>x</m>-direction along the curve of intersection of
the surfaces <m>G(x,y,z)=25</m> and <m>H(x,y,z)=0</m> where
<me>
G(x,y,z)=2x^2-y^2+2z^2 \qquad\text{and}\qquad
H(x,y,z)=x^2-y^2+z^2
</me>
</p>
</statement>

<solution>
<p>
As a first check note that <m>(3,5,4)</m>
really does lie on both surfaces because
<md alignment="alignat">
<mrow>
G(3,5,4)&amp;= 2\big(3^2\big)-5^2+2\big(4^2\big) &amp;&amp;= 18-25+32=25
</mrow><mrow>
H(3,5,4)&amp;=\phantom{2*\ }3^2-5^2+\phantom{2*}4^2&amp;&amp;=\phantom{1}9-25+16 =0
</mrow>
</md>
We compute gradients to get the normal vectors to the surfaces
<m>G(x,y,z)=25</m> and <m>H(x,y,z)=0</m> at <m>(3,5,4)</m>.
<md>
<mrow>
\vnabla G(3,5,4) &amp;=\Big[4x\,\hi-2y\,\hj+4z\,\hk\Big]_{(3,5,4)}
</mrow><mrow>    &amp;= 12\,\hi-10\,\hj+16\,\hk
                 = 2\big(6\,\hi-5\,\hj+8\,\hk\big)
</mrow><mrow>
\vnabla H(3,5,4) &amp;=\Big[2x\,\hi-2y\,\hj+2z\,\hk\Big]_{(3,5,4)}
</mrow><mrow>    &amp;= 6\,\hi-10\,\hj+8\,\hk
                 = 2\big(3\,\hi-5\,\hj+4\,\hk\big)
</mrow>
</md>
The direction of interest is tangent to the curve of intersection.
So the direction of interest is tangent to both surfaces and hence is
perpendicular to both gradients. Consequently one tangent vector to the
curve at <m>(3,5,4)</m> is
<md>
<mrow>
\vnabla G(3,5,4)\,\times  \vnabla H(3,5,4)
&amp;=4\big(6\,\hi-5\,\hj+8\,\hk\big)\times\big(3\,\hi-5\,\hj+4\,\hk\big)
</mrow><mrow>
&amp;=4\ \det\left[\begin{matrix}
             \hi &amp; \hj &amp; \hk \\
             6   &amp; -5  &amp; 8 \\
             3   &amp; -5  &amp; 4 \\
           \end{matrix}\right]
</mrow><mrow>
&amp;= 4\ \big(20\,\hi -15\,\hk\big)
= 20\ \big(4\,\hi -3\,\hk\big)
</mrow>
</md>
and the unit tangent vector to the curve at <m>(3,5,4)</m> that has
positive <m>x</m> component is
<me>
\frac{4\,\hi -3\,\hk}{|4\,\hi -3\,\hk|}
=\frac{4}{5}\,\hi -\frac{3}{5}\,\hk
</me>
The desired rate of change is
<md>
<mrow>
D_{\frac{4}{5}\,\hi -\frac{3}{5}\,\hj} f(3,5,4)
   &amp;= \vnabla f(3,5,4)\cdot\left(\frac{4}{5}\,\hi -\frac{3}{5}\,\hk\right)
</mrow><mrow>
   &amp;= \overbrace{\big( 6\,\hi +10\, \hj + 8\,\hk\big)}^
              {[2x\,\hi+2y\,\hj+2z\,\hk]_{(x,y,z)=(3,5,4)}}\hskip-0.15in\cdot\,
         \left(\frac{4}{5}\,\hi -\frac{3}{5}\,\hk\right)
</mrow><mrow>
  &amp;=0
</mrow>
</md>
Actually, we could have known that the rate of change would be zero.
<ul>
<li>indent=-0.1in
</li>
<li>
Any point <m>(x,y,z)</m> on the curve obeys both <m>y^2=x^2+z^2</m>
      and <m>2x^2-y^2+2z^2=25</m>.
</li>
<li>
Substituting <m>y^2=x^2+z^2</m> into <m>2x^2-y^2+2z^2=25</m> gives <m>x^2+z^2=25</m>.
</li>
<li>
So, at any point on the curve, <m>x^2+z^2=25</m> and <m>y^2=x^2+z^2=25</m> so
that <m>x^2+y^2+z^2=50</m>.
</li>
<li>
That is, <m>f(x,y,z)=x^2+y^2+z^2</m> takes the value 50 at every point of the curve.
</li>
<li>
So of course the rate of change of <m>f</m> along the curve is <m>0</m>.
</li>
</ul>
</p>
</solution>
</example>

<p>Let's change things up a little. In the next example, we are told the rates of change in two different directions. From this we are to determine the rate of change in a third direction.
</p>

<example xml:id="eg_dir_deriv_E">
<statement>
<p>
The rate of change of a given function <m>f(x,y)</m> at the point <m>P_0=(1,2)</m>
in the direction towards <m>P_1=(2,3)</m> is <m>2\sqrt{2}</m> and in the direction
towards <m>P_2=(1,0)</m> is <m>-3</m>. What is the rate of change of <m>f</m> at <m>P_0</m>
towards the origin <m>P_3=(0,0)</m>?
</p>
</statement>

<solution>
<p>
We can easily determine the rate of change of <m>f</m> at the point <m>P_0</m>
in any direction once we know the gradient <m>\vnabla f(1,2) =a\,\hi+b\,\hj</m>.
So we will first use the two given rates of change to determine <m>a</m> and <m>b</m>,
and then we determine the rate of change towards <m>(0,0)</m>.
</p>

<p>The two rates of change that we are given are those in the directions
of the vectors
<md>
<mrow>
\overrightarrow{P_0P_1} = \llt 1,1\rgt \qquad
\overrightarrow{P_0P_2} = \llt 0,-2\rgt
</mrow>
</md>
As you might guess, the notation <m>\overrightarrow{PQ}</m> means the
vector whose tail is at <m>P</m> and whose head is at <m>Q</m>.
So the given rates of change tell us that
<md alignment="alignat">
<mrow>
\sqrt{2}&amp;=D_{\frac{\llt 1,1\rgt}{|\llt 1,1\rgt|}} f(1,2)
   &amp;&amp;= \vnabla f(1,2)\cdot\frac{\llt 1,1\rgt}{|\llt 1,1\rgt|}
   &amp;&amp;= \llt a,b\rgt\cdot\frac{\llt 1,1\rgt}{\sqrt{2}}
</mrow><mrow>
   &amp;=\frac{a}{\sqrt{2}} +\frac{b}{\sqrt{2}}
</mrow><mrow>
-3&amp;=D_{\frac{\llt 0,-2\rgt}{|\llt 0,-2\rgt|}} f(1,2)
   &amp;&amp;= \vnabla f(1,2)\cdot\frac{\llt 0,-2\rgt}{|\llt 0,-2\rgt|}
   &amp;&amp;= \llt a,b\rgt\cdot\frac{\llt 0,-2\rgt}{2}
</mrow><mrow>
   &amp;=-b
</mrow>
</md>
These two lines give us two linear equations in the two unknowns <m>a</m> and <m>b</m>.
The second equation directly gives us <m>b=3</m>. Substituting <m>b=3</m> into
the first equation gives
<md>
<mrow>
\frac{a}{\sqrt{2}} +\frac{3}{\sqrt{2}} = 2\sqrt{2} \implies
a+3=4 \implies
a=1
</mrow>
</md>
A direction vector from <m>P_0=(1,2)</m> towards <m>P_3=(0,0)</m> is
<me>
\overrightarrow{P_0P_3} = \llt -1,-2\rgt
</me>
and the rate of change (per unit distance) in that direction is
<md>
<mrow>
D_{\frac{\llt -1,-2\rgt}{|\llt -1,-2\rgt|}} f(1,2)
   &amp;= \vnabla f(1,2)\cdot\frac{\llt -1,-2\rgt}{|\llt -1,-2\rgt|}
    = \llt a,b\rgt\cdot\frac{\llt -1,-2\rgt}{\sqrt{5}}
</mrow><mrow>
    &amp;= \llt 1,3\rgt\cdot\frac{\llt -1,-2\rgt}{\sqrt{5}}
=-\frac{7}{\sqrt{5}}
</mrow>
</md>
</p>
</solution>
</example>

<example xml:id="eg_dir_deriv_F"><title>Optional</title>
<statement>
<p>
Find all points <m>(a,b,c)</m> for which the spheres
<m>(x-a)^2+(y-b)^2+(z-c)^2 =1</m> and <m>x^2+y^2+z^2=1</m> intersect
orthogonally. That is, the tangent planes to the two spheres are
to be perpendicular at each point of intersection.
</p>
</statement>

<solution>
<p>
Let <m>(x_0,y_0,z_0)</m> be a point of intersection. That is
<md>
<mrow>
(x_0-a)^2+(y_0-b)^2+(z_0-c)^2 &amp; = 1
</mrow><mrow>
x_0^2+y_0^2+z_0^2&amp;=1
</mrow>
</md>
A normal vector to <m>G(x,y,z)=(x-a)^2+(y-b)^2+(z-c)^2 =1</m> at <m>(x_0,y_0,z_0)</m>
is
<me>
\vN = \vnabla G(x_0,y_0,z_0)
     = \llt 2(x_0-a)\,\hi\,,\,2(y_0-b)\,\hj\,,\,2(z_0-c)\,\hk\rgt
</me>
A normal vector to <m>g(x,y,z)=x^2+y^2+z^2 =1</m> at <m>(x_0,y_0,z_0)</m>
is
<me>
\vn = \vnabla g(x_0,y_0,z_0)
     = \llt 2x_0\,\hi\,,\,2y_0\,\hj\,,\,2z_0\,\hk\rgt
</me>
The two tangent planes are perpendicular if and only if <m>\hN</m> and <m>\hn</m>
are perpendicular, which is the case if and only if
<me>
0=\hN\cdot\hn = 4x_0(x_0-a) + 4y_0(y_0-b) +4z_0(z_0-c)
</me>
or, dividing the equation by <m>4</m>,
<me>
x_0(x_0-a) + y_0(y_0-b) +z_0(z_0-c)=0
</me>
</p>

<p>Let's pause to take stock.
We need to find all <m>(a,b,c)</m>'s such that the statement
<me>
(x_0,y_0,z_0)\text{ is a point of intersection of the two spheres}
\tag{S1}</me>
implies the statement
<me>
\text{the normal vectors $\hN$ and $\hn$ are perpendicular}
\tag{S2}</me>
In equations, we need to find all <m>(a,b,c)</m>'s such that the statement
<md>
<mrow>
(x_0,y_0,z_0)\quad\text{obeys}\quad
&amp;x_0^2+y_0^2+z_0^2 = 1
</mrow><mrow>
&amp;\text{ and }(x_0-a)^2+(y_0-b)^2+(z_0-c)^2 = 1
\tag{S1}
</mrow>
</md>
implies the statement
<me>
(x_0,y_0,z_0)\quad\text{obeys}\quad
x_0(x_0-a) + y_0(y_0-b) +z_0(z_0-c)=0
\tag{S2}
</me>
Now if we expand (S2) then we can, with a little care, massage it into something that looks more like (S1).
<md>
<mrow>
&amp;x_0(x_0-a) + y_0(y_0-b) +z_0(z_0-c)
=x_0^2+y_0^2+z_0^2 -ax_0 -by_0 - cz_0
</mrow><mrow>
&amp;=\frac{1}{2}\left\{\big[x_0^2+y_0^2+z_0^2\big]
     +\big[(x_0-a)^2+(y_0-b)^2+(z_0-c)^2\big]
     -a^2-b^2-c^2\right\}
</mrow>
</md>
If (S1) is true, then <m>\big[x_0^2+y_0^2+z_0^2\big]=1</m>
and <m>\big[(x_0-a)^2+(y_0-b)^2+(z_0-c)^2\big]=1</m> so that
<me>
x_0(x_0-a) + y_0(y_0-b) +z_0(z_0-c)
=\frac{1}{2}\left\{1 \ +\  1\  -a^2-b^2-c^2 \right\}
</me>
and statement (S2) is true if and only if
<me>
a^2+b^2+c^2=2
</me>
</p>

<p>Our conclusion is that the set of allowed points <m>(a,b,c)</m> is the
sphere of radius <m>\sqrt{2}</m> centred on the origin.
</p>
</solution>
</example>

<example xml:id="eg_chainRuleF"><title>Optional <mdash/> The gradient in polar coordinates</title>
<statement>
<p>
What is the gradient of a function in polar coordinates?
</p>
</statement>


<solution>
<p>
As was the case in Examples <xref ref="eg_chainRuleD"/> and <xref ref="eg_chainRuleE"/>, figuring
out what the question is asking is half the battle. By Definition
<xref ref="def_gradient"/>, the gradient of a function <m>g(x,y)</m>
is the vector <m>\llt g_x(x,y),g_y(x,y)\rgt</m>. In this question we are told
that we are given some function <m>f(r,\theta)</m> of the polar
coordinates
<fn>Polar coordinates were defined in
Example <xref ref="ex_LIMtwodB"/>.</fn>
 <m>r</m> and <m>\theta</m>. We are supposed to convert
this function to Cartesian  coordinates.
</p>

<p>This means that we are to consider the function
<me>
g(x,y)=f\big(r(x,y),\theta(x,y)\big)
</me>
with
<md>
<mrow>
r(x,y)&amp;=\sqrt{x^2+y^2}\cr
\theta(x,y)&amp;= \arctan\,\frac{y}{x}
</mrow>
</md>
Then we are to compute the gradient of <m>g(x,y)</m> and express the answer
in terms of <m>r</m> and <m>\theta</m>. By the chain rule,
<md>
<mrow>
\pdiff{g}{x}
&amp;=\pdiff{f}{r}\ \pdiff{r}{x}
           +\pdiff{f}{\theta}\  \pdiff{\theta}{x}
</mrow><mrow>
&amp;=\pdiff{f}{r}\ \frac{1}{2}\frac{2x}{\sqrt{x^2+y^2}}
        +\pdiff{f}{\theta}\ \frac{-y/x^2}{1+(y/x)^2}
</mrow><mrow>
&amp;=\pdiff{f}{r}\ \frac{x}{\sqrt{x^2+y^2}}
        -\pdiff{f}{\theta}\ \frac{y}{x^2+y^2}
</mrow><mrow>
&amp;=\pdiff{f}{r}\ \frac{r\cos\theta}{r}
       -\pdiff{f}{\theta}\ \frac{r\sin\theta}{r^2}
</mrow><mrow>
</mrow>
<intertext>since <m>x=r\cos\theta</m> and <m>y=r\sin\theta</m></intertext><mrow>
&amp;=\pdiff{f}{r}\ \cos\theta
           -\pdiff{f}{\theta}\ \frac{\sin\theta}{r}
</mrow>
</md>
Similarly
<md>
<mrow>
\pdiff{g}{y}
&amp;=\pdiff{f}{r}\ \pdiff{r}{y}
           +\pdiff{f}{\theta}\ \pdiff{\theta}{y}
</mrow><mrow>
&amp;=\pdiff{f}{r}\ \frac{1}{2}\frac{2y}{\sqrt{x^2+y^2}}
         +\pdiff{f}{\theta}\ \frac{1/x}{1+(y/x)^2}
</mrow><mrow>
&amp;=\pdiff{f}{r}\ \frac{y}{\sqrt{x^2+y^2}}
           +\pdiff{f}{\theta}\ \frac{x}{x^2+y^2}
</mrow><mrow>
&amp;=\pdiff{f}{r}\ \sin\theta
     +\pdiff{f}{\theta}\ \frac{\cos\theta}{r}
</mrow>
</md>
So
<me>
\llt g_x,g_y\rgt= f_r\ \llt\cos\theta,\sin\theta\rgt
           +\frac{f_\theta}{r}\llt-\sin\theta,\cos\theta\rgt
</me>
or, with all the arguments written explicitly,
<md>
<mrow>
\llt g_x(x,y),g_y(x,y)\rgt
&amp;=
f_r\big(r(x,y),\theta(x,y)\big)\ \llt\cos\theta(x,y)\,,\,\sin\theta(x,y)\rgt
</mrow><mrow>
&amp;\ \ +\frac{1}{r(x,y)}f_\theta\big(r(x,y),\theta(x,y)\big)\
\llt-\sin\theta(x,y)\,,\,\cos\theta(x,y)\rgt
</mrow>
</md>
</p>
</solution>
</example>
</subsubsection>
</subsection>
<xi:include href="../problems/prob_s2.7.ptx" />

</section>
